@prefix skos: <http://www.w3.org/2004/02/skos/core#> .

<http://historyofwork.iisg.nl/resource/01110> a skos:Concept ;
    skos:broader <http://historyofwork.iisg.nl/resource/011> ;
    skos:definition "Conducts chemical experiments, tests and analyses to investigate chemical phenomena, to test, develop or improve materials and products and to control or develop industrial processes."@en ;
    skos:prefLabel "Chemist, General"@en .

<http://historyofwork.iisg.nl/resource/01120> a skos:Concept ;
    skos:broader <http://historyofwork.iisg.nl/resource/011> ;
    skos:definition "Conducts chemical experiments, tests and analyses on substances of which main element is carbon, to investigate chemical phenomena, to test, develop or improve materials and products or to control or develop industrial processes."@en ;
    skos:prefLabel "Organic Chemist"@en .

<http://historyofwork.iisg.nl/resource/01130> a skos:Concept ;
    skos:broader <http://historyofwork.iisg.nl/resource/011> ;
    skos:definition "Conducts chemical experiments, tests and analyses on substances free or relatively free of carbon to investigate chemical phenomena, to test, develop or improve materials and products, or to control or develop industrial processes."@en ;
    skos:prefLabel "Inorganic Chemist"@en .

<http://historyofwork.iisg.nl/resource/01140> a skos:Concept ;
    skos:broader <http://historyofwork.iisg.nl/resource/011> ;
    skos:definition "Conducts research into relationships between chemical and physical properties of substances to increase knowledge of physical aspects of chemical phenomena or to develop or improve materials, products or industrial processes."@en ;
    skos:prefLabel "Physical Chemist"@en .

<http://historyofwork.iisg.nl/resource/01150> a skos:Concept ;
    skos:broader <http://historyofwork.iisg.nl/resource/011> ;
    skos:definition "Carries out chemical tests and analyses of substances and develops and improves analytical methodology and techniques."@en ;
    skos:prefLabel "Analytical Chemist"@en .

<http://historyofwork.iisg.nl/resource/01190> a skos:Concept ;
    skos:broader <http://historyofwork.iisg.nl/resource/011> ;
    skos:definition "This group includes chemists not elsewhere classified, for example those who specialise in the development and technical control of the manufacture of pharmaceutical products. Pharmacologist is classified in 0-52.70 and Pharmacist in 0-67.10."@en ;
    skos:prefLabel "Other Chemists"@en .

<http://historyofwork.iisg.nl/resource/01210> a skos:Concept ;
    skos:broader <http://historyofwork.iisg.nl/resource/012> ;
    skos:definition "Conducts research into physical phenomena to increase scientific knowledge and to develop and improve materials, products and industrial and other processes."@en ;
    skos:prefLabel "Physicist, General"@en .

<http://historyofwork.iisg.nl/resource/01220> a skos:Concept ;
    skos:broader <http://historyofwork.iisg.nl/resource/012> ;
    skos:definition "Conducts research in the field of mechanics to investigate physical phenomena or to develop or improve materials, products or industrial and other processes."@en ;
    skos:prefLabel "Mechanics Physicist"@en .

<http://historyofwork.iisg.nl/resource/01230> a skos:Concept ;
    skos:broader <http://historyofwork.iisg.nl/resource/012> ;
    skos:definition "Conducts research into nature and effects of heat to increase scientific knowledge or to develop or improve materials, products or industrial and other processes."@en ;
    skos:prefLabel "Heat Physicist"@en .

<http://historyofwork.iisg.nl/resource/01240> a skos:Concept ;
    skos:broader <http://historyofwork.iisg.nl/resource/012> ;
    skos:definition "Conducts research into nature and effects of light to increase scientific knowledge or to develop or improve materials, products or industrial and other processes."@en ;
    skos:prefLabel "Light Physicist"@en .

<http://historyofwork.iisg.nl/resource/01250> a skos:Concept ;
    skos:broader <http://historyofwork.iisg.nl/resource/012> ;
    skos:definition "Conducts research into nature and effects of sound to increase scientific knowledge or to develop or improve materials, products or industrial and other processes."@en ;
    skos:prefLabel "Sound Physicist"@en .

<http://historyofwork.iisg.nl/resource/01260> a skos:Concept ;
    skos:broader <http://historyofwork.iisg.nl/resource/012> ;
    skos:definition "Conducts research into nature and properties of electricity and magnetism to increase scientific knowledge or to develop or improve materials, products or industrial and other processes."@en ;
    skos:prefLabel "Electricity and Magnetism Physicist"@en .

<http://historyofwork.iisg.nl/resource/01270> a skos:Concept ;
    skos:broader <http://historyofwork.iisg.nl/resource/012> ;
    skos:definition "Conducts research into nature and behaviour of electrons to increase scientific knowledge or to develop or improve materials, products or industrial or other processes."@en ;
    skos:prefLabel "Electronics Physicist"@en .

<http://historyofwork.iisg.nl/resource/01280> a skos:Concept ;
    skos:broader <http://historyofwork.iisg.nl/resource/012> ;
    skos:definition "Conducts research into structure and characteristics of atoms, molecules and nuclei to increase scientific knowledge or to discover practical applications of atomic, molecular and nuclear physics."@en ;
    skos:prefLabel "Nuclear Physicist"@en .

<http://historyofwork.iisg.nl/resource/01290> a skos:Concept ;
    skos:broader <http://historyofwork.iisg.nl/resource/012> ;
    skos:definition "This group includes physicists not elsewhere classified, for example those who conduct research into structure and properties of matter in solid state; or specialise in pure research and formulate theories based on analysis of established data to explain relationships between observed physical phenomena and to explain previously unobserved phenomena, or predict results of experiments designed to detect and measure them."@en ;
    skos:prefLabel "Other Physicists"@en .

<http://historyofwork.iisg.nl/resource/01320> a skos:Concept ;
    skos:broader <http://historyofwork.iisg.nl/resource/013> ;
    skos:definition "Conducts research into physical nature of earth, including its atmosphere and hydrosphere, to increase scientific knowledge and to develop practical applications in such fields as radio communications, water conservation, volcanology and mineral exploration."@en ;
    skos:prefLabel "Geophysical Scientist"@en .

<http://historyofwork.iisg.nl/resource/01330> a skos:Concept ;
    skos:broader <http://historyofwork.iisg.nl/resource/013> ;
    skos:definition "Conducts research into nature and history of earth's crust to increase scientific knowledge and to develop practical applications in such fields as mineral exploitation and civil engineering."@en ;
    skos:prefLabel "Geological Scientist"@en .

<http://historyofwork.iisg.nl/resource/01340> a skos:Concept ;
    skos:broader <http://historyofwork.iisg.nl/resource/013> ;
    skos:definition "Conducts research into physical nature and properties of the earth's atmosphere and the forces affecting it to increase scientific knowledge and to develop practical applications such as weather forecasts."@en ;
    skos:prefLabel "Meteorological Scientist"@en .

<http://historyofwork.iisg.nl/resource/01350> a skos:Concept ;
    skos:broader <http://historyofwork.iisg.nl/resource/013> ;
    skos:definition "Observes and interprets celestial phenomena to increase scientific knowledge and to develop practical applications in such fields as navigation and space exploration."@en ;
    skos:prefLabel "Astronomical Scientist"@en .

<http://historyofwork.iisg.nl/resource/01390> a skos:Concept ;
    skos:broader <http://historyofwork.iisg.nl/resource/013> ;
    skos:definition "This group includes other physical scientists not elsewhere classified, for example those who specialise in examining, analysing and classifying minerals (including gems and precious stones) or advising on the likely commercial yield from mineral deposits containing gems and precious stones."@en ;
    skos:prefLabel "Other Physical Scientists"@en .

<http://historyofwork.iisg.nl/resource/01400> a skos:Concept ;
    skos:broader <http://historyofwork.iisg.nl/resource/014> ;
    skos:definition "May perform any (but not all) of the occupational activities described in unit group 0-14."@en ;
    skos:prefLabel "Physical Science Technician, Specialisation Unknown"@en .

<http://historyofwork.iisg.nl/resource/01420> a skos:Concept ;
    skos:broader <http://historyofwork.iisg.nl/resource/014> ;
    skos:definition "Performs auxiliary technical tasks, normally under direction and supervision of chemist, in connection with pure research into chemical phenomena or applied chemical research and development work."@en ;
    skos:prefLabel "Chemistry Technician"@en .

<http://historyofwork.iisg.nl/resource/01430> a skos:Concept ;
    skos:broader <http://historyofwork.iisg.nl/resource/014> ;
    skos:definition "Performs auxiliary technical tasks, normally under direction of physicist, in connection with pure research into physical phenomena or applied physics research and development work."@en ;
    skos:prefLabel "Physics Technician"@en .

<http://historyofwork.iisg.nl/resource/01490> a skos:Concept ;
    skos:broader <http://historyofwork.iisg.nl/resource/014> ;
    skos:definition "This group includes physical science technicians not elsewhere classified, for example those who perform auxiliary technical tasks in connection with research and development work conducted by geological, geophysical meteorological and astronomic scientists."@en ;
    skos:prefLabel "Other Physical Science Technicians"@en .

<http://historyofwork.iisg.nl/resource/02000> a skos:Concept ;
    skos:broader <http://historyofwork.iisg.nl/resource/020> ;
    skos:definition "May perform any (but not all) of the occupational activities listed in unit groups 0-22 to 0-29."@en ;
    skos:prefLabel "Engineers, Specialisation Unknown"@en .

<http://historyofwork.iisg.nl/resource/02120> a skos:Concept ;
    skos:broader <http://historyofwork.iisg.nl/resource/021> ;
    skos:definition "Designs buildings and exercises general supervision over their construction. Building construction engineer is classified in 0-22.20."@en ;
    skos:prefLabel "Building Architect"@en .

<http://historyofwork.iisg.nl/resource/02130> a skos:Concept ;
    skos:broader <http://historyofwork.iisg.nl/resource/021> ;
    skos:definition "Plans layout and co-ordinates development of urban areas."@en ;
    skos:prefLabel "Town Planner"@en .

<http://historyofwork.iisg.nl/resource/02140> a skos:Concept ;
    skos:broader <http://historyofwork.iisg.nl/resource/021> ;
    skos:definition "Plans and designs aesthetic layout of land areas for such projects as parks and other recreational facilities, roads, commercial, industrial and residential sites and public buildings."@en ;
    skos:prefLabel "Landscape Architect"@en .

<http://historyofwork.iisg.nl/resource/02210> a skos:Concept ;
    skos:broader <http://historyofwork.iisg.nl/resource/022> ;
    skos:definition "Carries out research, designs and advises on structures such as bridges, dams, docks, roads, airports, railways, waste disposal and flood control systems and industrial and other large buildings, and plans, organises and supervises their construction, maintenance and repair."@en ;
    skos:prefLabel "Civil Engineer, General"@en .

<http://historyofwork.iisg.nl/resource/02220> a skos:Concept ;
    skos:broader <http://historyofwork.iisg.nl/resource/022> ;
    skos:definition "Designs structures of large buildings and plans, organises and supervises their erection, maintenance and repair."@en ;
    skos:prefLabel "Building Construction Engineer"@en .

<http://historyofwork.iisg.nl/resource/02230> a skos:Concept ;
    skos:broader <http://historyofwork.iisg.nl/resource/022> ;
    skos:definition "Designs highways and streets and plans, organises and supervises their construction, maintenance and repair."@en ;
    skos:prefLabel "Highway and Street Construction Engineer"@en .

<http://historyofwork.iisg.nl/resource/02235> a skos:Concept ;
    skos:broader <http://historyofwork.iisg.nl/resource/022> ;
    skos:definition "Designs airports and landing strips and plans, organises and supervises their construction, maintenance and repair."@en ;
    skos:prefLabel "Aerodrome Construction Engineer"@en .

<http://historyofwork.iisg.nl/resource/02240> a skos:Concept ;
    skos:broader <http://historyofwork.iisg.nl/resource/022> ;
    skos:definition "Designs railroads, terminals and other railway structures and plans, organises and supervises their construction, maintenance and repair."@en ;
    skos:prefLabel "Railway Construction Engineer"@en .

<http://historyofwork.iisg.nl/resource/02245> a skos:Concept ;
    skos:broader <http://historyofwork.iisg.nl/resource/022> ;
    skos:definition "Designs bridges and plans, organises and supervises their construction, maintenance and repair."@en ;
    skos:prefLabel "Bridge Construction Engineer"@en .

<http://historyofwork.iisg.nl/resource/02250> a skos:Concept ;
    skos:broader <http://historyofwork.iisg.nl/resource/022> ;
    skos:definition "Designs engineering structures and equipment related to public health and hygiene, such as are required for water-supply and waste-disposal systems, and plans, organises and supervises their construction, operation, maintenance and repair."@en ;
    skos:prefLabel "Sanitary Engineer"@en .

<http://historyofwork.iisg.nl/resource/02255> a skos:Concept ;
    skos:broader <http://historyofwork.iisg.nl/resource/022> ;
    skos:definition "Designs hydro-power, water supply, irrigation, inland waterways and related projects and plans, organises and supervises their construction, maintenance and repair."@en ;
    skos:prefLabel "Hydraulics Engineer"@en .

<http://historyofwork.iisg.nl/resource/02260> a skos:Concept ;
    skos:broader <http://historyofwork.iisg.nl/resource/022> ;
    skos:definition "Examines soils and ascertains their effect on construction work and suitability as building materials."@en ;
    skos:prefLabel "Soil Mechanics Engineer"@en .

<http://historyofwork.iisg.nl/resource/02290> a skos:Concept ;
    skos:broader <http://historyofwork.iisg.nl/resource/022> ;
    skos:definition "This group includes civil engineers not elsewhere classified, for example those who perform tasks similar to those of Civil engineer, general (0-22.10) but specialise in the design, construction and maintenance of tunnels, wharves, docks and harbour breakwaters, lighthouses, chimney stacks, towers and pylons; or in the dredging of harbours and ship channels."@en ;
    skos:prefLabel "Other Civil Engineers"@en .

<http://historyofwork.iisg.nl/resource/02305> a skos:Concept ;
    skos:broader <http://historyofwork.iisg.nl/resource/023> ;
    skos:definition "Carries out research on electrical engineering problems, designs and advises on electrical systems and equipment, and plans and supervises their development, construction, installation, operation, maintenance and repair."@en ;
    skos:prefLabel "Electrical Engineer, General"@en .

<http://historyofwork.iisg.nl/resource/02310> a skos:Concept ;
    skos:broader <http://historyofwork.iisg.nl/resource/023> ;
    skos:definition "Carries out research on electronics engineering problems, designs and advises on electronic devices and equipment and plans and supervises their development, construction, installation, operation, maintenance and repair."@en ;
    skos:prefLabel "Electronics Engineer, General"@en .

<http://historyofwork.iisg.nl/resource/02320> a skos:Concept ;
    skos:broader <http://historyofwork.iisg.nl/resource/023> ;
    skos:definition "Studies, designs and advises on electricity generating systems and plant and plans and supervises their construction, operation, maintenance and repair."@en ;
    skos:prefLabel "Power Generation Engineer"@en .

<http://historyofwork.iisg.nl/resource/02330> a skos:Concept ;
    skos:broader <http://historyofwork.iisg.nl/resource/023> ;
    skos:definition "Studies, designs and advises on systems and equipment for transmission and distribution of electric power and plans and supervises their development, construction, maintenance and repair."@en ;
    skos:prefLabel "Power Distribution and Transmission Engineer"@en .

<http://historyofwork.iisg.nl/resource/02340> a skos:Concept ;
    skos:broader <http://historyofwork.iisg.nl/resource/023> ;
    skos:definition "Studies, designs and advises on telecommunication systems and equipment and plans and supervises their development, construction, installation, operation, maintenance and repair."@en ;
    skos:prefLabel "Telecommunications Engineer"@en .

<http://historyofwork.iisg.nl/resource/02390> a skos:Concept ;
    skos:broader <http://historyofwork.iisg.nl/resource/023> ;
    skos:definition "This group includes electrical and electronics engineers not elsewhere classified, for example those who perform tasks similar to those of Electrical engineer, general (0-23.05) or Electronics engineer, general (0-23.10) but specialise in the design, production, operation or maintenance of particular apparatus or products such as electronic calculating and data-processing equipment; radar, radio or television; signalling and automatic control systems; electric traction equipment; electric motors; domestic electrical appliances; or other electrical or electronic apparatus (excluding power generation, transmission and distribution and telecommunications equipment)."@en ;
    skos:prefLabel "Other Electrical and Electronics Engineers"@en .

<http://historyofwork.iisg.nl/resource/02410> a skos:Concept ;
    skos:broader <http://historyofwork.iisg.nl/resource/024> ;
    skos:definition "Carries out research on, designs and advises on mechanically functioning plant and equipment, and plans and supervises their development, manufacture, construction, installation, operation, maintenance and repair."@en ;
    skos:prefLabel "Mechanical Engineer, General"@en .

<http://historyofwork.iisg.nl/resource/02420> a skos:Concept ;
    skos:broader <http://historyofwork.iisg.nl/resource/024> ;
    skos:definition "Studies, designs and advises on machinery and tools for manufacturing, mining, construction, agricultural work, printing and other industrial purposes, and plans and supervises their development, manufacture, installation, operation, maintenance and repair."@en ;
    skos:prefLabel "Industrial Machinery and Tools Engineer"@en .

<http://historyofwork.iisg.nl/resource/02430> a skos:Concept ;
    skos:broader <http://historyofwork.iisg.nl/resource/024> ;
    skos:definition "Studies, designs and advises on steam, internal combustion and other non-electric motors and engines as used for propulsion of railway locomotives, road vehicles or aeroplanes, or for driving industrial and other machinery, and plans and supervises their development, manufacture, installation, maintenance and repair. Engineers specialising in electric motors are classified in 0-23.90."@en ;
    skos:prefLabel "Mechanical Engineer (Motors and Engines, except Marine)"@en .

<http://historyofwork.iisg.nl/resource/02440> a skos:Concept ;
    skos:broader <http://historyofwork.iisg.nl/resource/024> ;
    skos:definition "Studies, designs and advises on ships' propulsion systems, power plants, heating and ventilating systems, steering gear, pumps and other mechanical and electrical equipment, and plans and supervises their development, construction, installation, maintenance and repair. A marine engineer who is a member of a ship's crew is classified in unit group 0-43."@en ;
    skos:prefLabel "Marine Engineer"@en .

<http://historyofwork.iisg.nl/resource/02450> a skos:Concept ;
    skos:broader <http://historyofwork.iisg.nl/resource/024> ;
    skos:definition "Studies, designs and advises on the hulls and superstructures of ships and other vessels, and plans and supervises their development, construction, maintenance and repair."@en ;
    skos:prefLabel "Ship Construction Engineer"@en .

<http://historyofwork.iisg.nl/resource/02460> a skos:Concept ;
    skos:broader <http://historyofwork.iisg.nl/resource/024> ;
    skos:definition "Studies, designs and advises on airframes, undercarriages and other equipment for aircraft, and plans and supervises their development, construction, maintenance and repair."@en ;
    skos:prefLabel "Aeronautical Engineer"@en .

<http://historyofwork.iisg.nl/resource/02470> a skos:Concept ;
    skos:broader <http://historyofwork.iisg.nl/resource/024> ;
    skos:definition "Studies, designs and advises on road vehicle bodies, suspension systems, brakes and other components, and plans and supervises their development and manufacture."@en ;
    skos:prefLabel "Automotive Engineer"@en .

<http://historyofwork.iisg.nl/resource/02480> a skos:Concept ;
    skos:broader <http://historyofwork.iisg.nl/resource/024> ;
    skos:definition "Studies, designs and advises on heating, ventilation and refrigeration systems and equipment, and plans and supervises their development, manufacture, installation, maintenance and repair."@en ;
    skos:prefLabel "Heating, Ventilation and Refrigeration Engineer"@en .

<http://historyofwork.iisg.nl/resource/02485> a skos:Concept ;
    skos:broader <http://historyofwork.iisg.nl/resource/024> ;
    skos:definition "Studies, designs and advises on mechanical plant and equipment for the release, control and utilisation of nuclear energy, and plans and supervises their development, manufacture, installation, maintenance and repair."@en ;
    skos:prefLabel "Nuclear Power Engineer"@en .

<http://historyofwork.iisg.nl/resource/02490> a skos:Concept ;
    skos:broader <http://historyofwork.iisg.nl/resource/024> ;
    skos:definition "This group includes mechanical engineers not elsewhere classified, for example those who perform tasks similar to those of Mechanical engineer, general (0-24.10) but specialise in the design, production or maintenance of particular apparatus or products such as precision instruments; cameras and projectors; typewriters, desk calculators, cash registers and ticket machines; duplicating and copying machines; mechanically functioning medical equipment; or special space vehicles and mechanical equipment for space exploration and travel."@en ;
    skos:prefLabel "Other Mechanical Engineers"@en .

<http://historyofwork.iisg.nl/resource/02510> a skos:Concept ;
    skos:broader <http://historyofwork.iisg.nl/resource/025> ;
    skos:definition "Carries out research on chemical engineering problems and develops and advises on processes for producing on a commercial scale the chemical or physical transformation of substances, as in the manufacture of chemicals, petroleum derivatives, metals, food products and synthetic materials, designs appropriate manufacturing plant and plans and supervises its construction, operation, maintenance and repair."@en ;
    skos:prefLabel "Chemical Engineer, General"@en .

<http://historyofwork.iisg.nl/resource/02520> a skos:Concept ;
    skos:broader <http://historyofwork.iisg.nl/resource/025> ;
    skos:definition "Studies, develops and advises on processes for the refining of crude oil, designs appropriate plant and plans and supervises its construction, operation, maintenance and repair."@en ;
    skos:prefLabel "Chemical Engineer (Petroleum)"@en .

<http://historyofwork.iisg.nl/resource/02590> a skos:Concept ;
    skos:broader <http://historyofwork.iisg.nl/resource/025> ;
    skos:definition "This group includes chemical engineers not elsewhere classified, for example those who perform tasks similar to those of Chemical engineer, general (0-25.10) but specialise in the development and efficient utilisation of fuels; the design, construction, operation and maintenance of plant for the physical and chemical transformation of matter for the manufacture of a particular type of commodity such as antibiotics, plastics, explosives, rubber or pigments, or of plant for production and distribution of fuel gas for industrial, domestic and other purposes."@en ;
    skos:prefLabel "Other Chemical Engineers"@en .

<http://historyofwork.iisg.nl/resource/02620> a skos:Concept ;
    skos:broader <http://historyofwork.iisg.nl/resource/026> ;
    skos:definition "Studies, develops, advises on and controls the application of processes for the extraction of metals from their ores."@en ;
    skos:prefLabel "Extractive Metallurgist"@en .

<http://historyofwork.iisg.nl/resource/02630> a skos:Concept ;
    skos:broader <http://historyofwork.iisg.nl/resource/026> ;
    skos:definition "Studies properties of metals and alloys, develops new alloys and advises on and supervises technical aspects of metal and alloy manufacture and processing."@en ;
    skos:prefLabel "Physical Metallurgist"@en .

<http://historyofwork.iisg.nl/resource/02690> a skos:Concept ;
    skos:broader <http://historyofwork.iisg.nl/resource/026> ;
    skos:definition "This group includes metallurgists not elsewhere classified, for example those who specialise in metallurgical problems of radioactive materials."@en ;
    skos:prefLabel "Other Metallurgists"@en .

<http://historyofwork.iisg.nl/resource/02710> a skos:Concept ;
    skos:broader <http://historyofwork.iisg.nl/resource/027> ;
    skos:definition "Carries out research on mining engineering problems, advises on the extraction of metallic and solid nonmetallic minerals from the earth, supervises mineral prospecting and plans, organises and supervises mineral mining operations and preparation of minerals for distribution or processing."@en ;
    skos:prefLabel "Mining Engineer, General"@en .

<http://historyofwork.iisg.nl/resource/02720> a skos:Concept ;
    skos:broader <http://historyofwork.iisg.nl/resource/027> ;
    skos:definition "Studies and advises on coal-mining engineering problems and plans, organises and supervises coal-mining operations and preparation of coal for distribution."@en ;
    skos:prefLabel "Coal-Mining Engineer"@en .

<http://historyofwork.iisg.nl/resource/02730> a skos:Concept ;
    skos:broader <http://historyofwork.iisg.nl/resource/027> ;
    skos:definition "Studies and advises on metal-mining engineering problems and plans, organises and supervises metal-mining operations and preparation of metallic ores for distribution or processing. Engineers who specialise in the extraction of minerals from alluvial deposits by sluicing or dredging are classified in 0-27.90."@en ;
    skos:prefLabel "Metal-Mining Engineer"@en .

<http://historyofwork.iisg.nl/resource/02740> a skos:Concept ;
    skos:broader <http://historyofwork.iisg.nl/resource/027> ;
    skos:definition "Studies and advises on petroleum and natural gas extraction engineering problems, and plans, organises and supervises the extraction, storage, intial treatment and transportation of petroleum and natural gas."@en ;
    skos:prefLabel "Petroleum and Natural Gas Engineer"@en .

<http://historyofwork.iisg.nl/resource/02790> a skos:Concept ;
    skos:broader <http://historyofwork.iisg.nl/resource/027> ;
    skos:definition "This group includes mining engineers not elsewhere classified, for example those who perform tasks similar to those of Mining engineer, general (0-27.10) but specialise in mining or quarrying solid minerals (other than coal and metallic minerals) such as stone, marble, clay, salt, gravel or diamonds; extracting subsurface water or sulphur and other solid minerals by drilling boreholes; or extracting tin, gold, diamonds or other solid minerals from alluvial deposits by sluicing and dredging."@en ;
    skos:prefLabel "Other Mining Engineers"@en .

<http://historyofwork.iisg.nl/resource/02810> a skos:Concept ;
    skos:broader <http://historyofwork.iisg.nl/resource/028> ;
    skos:definition "Studies and advises on the organisation of production processes and commercial and administrative procedures, plans and supervises time and motion studies and makes recommendations to promote efficiency and supervises their implementation."@en ;
    skos:prefLabel "Industrial Efficiency Engineer, General"@en .

<http://historyofwork.iisg.nl/resource/02820> a skos:Concept ;
    skos:broader <http://historyofwork.iisg.nl/resource/028> ;
    skos:definition "Analyses industrial, commercial and other projects and administrative procedures, makes recommendations regarding organisation, methods of work and sequence of operations and supervises their implementation."@en ;
    skos:prefLabel "Methods Engineer"@en .

<http://historyofwork.iisg.nl/resource/02830> a skos:Concept ;
    skos:broader <http://historyofwork.iisg.nl/resource/028> ;
    skos:definition "Studies, develops and advises on work measurement procedures, plans and supervises time and motion studies, makes recommendations to promote efficiency and supervises their implementation."@en ;
    skos:prefLabel "Time and Motion Study Engineer"@en .

<http://historyofwork.iisg.nl/resource/02890> a skos:Concept ;
    skos:broader <http://historyofwork.iisg.nl/resource/028> ;
    skos:definition "This group includes industrial engineers not elsewhere classified, for example those who specialise in the prevention of industrial accidents and diseases by identifying potential hazards and developing and introducing safety procedures and devices, and those who specialise in the efficient layout of industrial plant or commercial establishments."@en ;
    skos:prefLabel "Other Industrial Engineers"@en .

<http://historyofwork.iisg.nl/resource/02920> a skos:Concept ;
    skos:broader <http://historyofwork.iisg.nl/resource/029> ;
    skos:definition "Carries out research and advises on, designs, develops and controls processes and plant for the manufacture of bricks, pottery and glassware."@en ;
    skos:prefLabel "Ceramics and Glass Technologist"@en .

<http://historyofwork.iisg.nl/resource/02930> a skos:Concept ;
    skos:broader <http://historyofwork.iisg.nl/resource/029> ;
    skos:definition "Studies and advises on the application of engineering technology to agricultural problems, designs agricultural machinery, structures and equipment and plans and supervises their manufacture, construction and installation. Engineers specialising in civil, mechanical or other particular types of engineering problems affecting the agricultural industry are classified elsewhere in minor group 0-2/0-3."@en ;
    skos:prefLabel "Agricultural Engineer"@en .

<http://historyofwork.iisg.nl/resource/02940> a skos:Concept ;
    skos:broader <http://historyofwork.iisg.nl/resource/029> ;
    skos:definition "Carries out research and advises on, designs, develops and controls processes and plant for the manufacture and processing of foods and beverages."@en ;
    skos:prefLabel "Food and Drink Technologist"@en .

<http://historyofwork.iisg.nl/resource/02950> a skos:Concept ;
    skos:broader <http://historyofwork.iisg.nl/resource/029> ;
    skos:definition "Studies, plans and advises on the routing and control of road traffic to promote safety and minimise congestion."@en ;
    skos:prefLabel "Traffic Planner"@en .

<http://historyofwork.iisg.nl/resource/02990> a skos:Concept ;
    skos:broader <http://historyofwork.iisg.nl/resource/029> ;
    skos:definition "This group includes engineers not elsewhere classified, for example those who study, design, develop, control and advise on processes and plant for the manufacture or processing of textiles, leather products, wood or paper."@en ;
    skos:prefLabel "Other Engineers"@en .

<http://historyofwork.iisg.nl/resource/03010> a skos:Concept ;
    skos:broader <http://historyofwork.iisg.nl/resource/030> ;
    skos:definition "Surveys earth's surface, natural topography and manmade structures, and underground areas to delineate features and determine exact locations and measurements for such purposes as mapmaking, construction work and mining."@en ;
    skos:prefLabel "Surveyor, General"@en .

<http://historyofwork.iisg.nl/resource/03020> a skos:Concept ;
    skos:broader <http://historyofwork.iisg.nl/resource/030> ;
    skos:definition "Surveys land surfaces to determine boundaries and exact locations, delineate topographic features and man-made structures and otherwise measure land areas for such purposes as mapmaking and construction work."@en ;
    skos:prefLabel "Land Surveyor"@en .

<http://historyofwork.iisg.nl/resource/03030> a skos:Concept ;
    skos:broader <http://historyofwork.iisg.nl/resource/030> ;
    skos:definition "Surveys mines and delineates surface and underground features to control direction and extent of mining."@en ;
    skos:prefLabel "Mine Surveyor"@en .

<http://historyofwork.iisg.nl/resource/03040> a skos:Concept ;
    skos:broader <http://historyofwork.iisg.nl/resource/030> ;
    skos:definition "Surveys sea, river and lake beds to delineate underwater topographic features for such purposes as chart making, determining navigable channels and planning construction and repair of harbours, piers, breakwaters and other marine structures."@en ;
    skos:prefLabel "Hydrographic Surveyor"@en .

<http://historyofwork.iisg.nl/resource/03050> a skos:Concept ;
    skos:broader <http://historyofwork.iisg.nl/resource/030> ;
    skos:definition "Analyses photographs and survey data to prepare and revise topographic maps and charts."@en ;
    skos:prefLabel "Photogrammetrist"@en .

<http://historyofwork.iisg.nl/resource/03090> a skos:Concept ;
    skos:broader <http://historyofwork.iisg.nl/resource/030> ;
    skos:definition "This group includes surveyors not elsewhere classified, for example those who specialise in planning and constructing aerial photographic surveys."@en ;
    skos:prefLabel "Other Surveyors"@en .

<http://historyofwork.iisg.nl/resource/03110> a skos:Concept ;
    skos:broader <http://historyofwork.iisg.nl/resource/031> ;
    skos:definition "Prepares accurate working plans and detailed drawings for engineering, construction, manufacturing or other projects, based on designer's sketches and specifications, and prepares charts and working drawings for other purposes."@en ;
    skos:prefLabel "Draughtsman, General"@en .

<http://historyofwork.iisg.nl/resource/03120> a skos:Concept ;
    skos:broader <http://historyofwork.iisg.nl/resource/031> ;
    skos:definition "Prepares engineering working drawings from designer's sketches and specifications for manufacture of machines, mechanical devices and related products."@en ;
    skos:prefLabel "Mechanical Draughtsman"@en .

<http://historyofwork.iisg.nl/resource/03130> a skos:Concept ;
    skos:broader <http://historyofwork.iisg.nl/resource/031> ;
    skos:definition "Prepares working drawings from designer's sketches and specifications for manufacture and installation of electrical and electronic machinery and equipment."@en ;
    skos:prefLabel "Electrical Draughtsman"@en .

<http://historyofwork.iisg.nl/resource/03140> a skos:Concept ;
    skos:broader <http://historyofwork.iisg.nl/resource/031> ;
    skos:definition "Prepares working drawings from designer's sketches and specifications for use in civil engineering projects."@en ;
    skos:prefLabel "Civil Engineering Draughtsman"@en .

<http://historyofwork.iisg.nl/resource/03150> a skos:Concept ;
    skos:broader <http://historyofwork.iisg.nl/resource/031> ;
    skos:definition "Prepares working drawings from architect's sketches and specifications for construction of buildings."@en ;
    skos:prefLabel "Architectural Draughtsman"@en .

<http://historyofwork.iisg.nl/resource/03160> a skos:Concept ;
    skos:broader <http://historyofwork.iisg.nl/resource/031> ;
    skos:definition "Prepares maps and charts from survey and other data."@en ;
    skos:prefLabel "Cartographical Draughtsman"@en .

<http://historyofwork.iisg.nl/resource/03170> a skos:Concept ;
    skos:broader <http://historyofwork.iisg.nl/resource/031> ;
    skos:definition "Draws technical illustrations for brochures, reference works and technical manuals dealing with assembly, installation, operation or use, maintenance and repair of machinery and other equipment."@en ;
    skos:prefLabel "Technical Illustrator"@en .

<http://historyofwork.iisg.nl/resource/03180> a skos:Concept ;
    skos:broader <http://historyofwork.iisg.nl/resource/031> ;
    skos:definition "Sketches designs in black and white or colour for preparation of lithographic stones, photo-engraving and other printing processes."@en ;
    skos:prefLabel "Lithographic Artist"@en .

<http://historyofwork.iisg.nl/resource/03190> a skos:Concept ;
    skos:broader <http://historyofwork.iisg.nl/resource/031> ;
    skos:definition "This group includes draughtsmen not elsewhere classified, for example those who specialise in preparing working drawings for the installation of heating and ventilating systems or preparing maps, diagrams, profiles and cross-sections to show geological stratigraphy and location of mineral deposits."@en ;
    skos:prefLabel "Other Draughtsmen"@en .

<http://historyofwork.iisg.nl/resource/03200> a skos:Concept ;
    skos:broader <http://historyofwork.iisg.nl/resource/032> ;
    skos:definition "May perform any (but not all) of the occupational activities described in unit groups 0-14 and 0-33 to 0-39."@en ;
    skos:prefLabel "Technician, Specialisation Unknown"@en .

<http://historyofwork.iisg.nl/resource/03310> a skos:Concept ;
    skos:broader <http://historyofwork.iisg.nl/resource/033> ;
    skos:definition "Performs technical tasks, normally under direction and supervision of civil engineer or building architect, contributory to planning and execution of building and civil engineering projects, including new construction, repair and maintenance."@en ;
    skos:prefLabel "Civil Engineering Technician, General"@en .

<http://historyofwork.iisg.nl/resource/03320> a skos:Concept ;
    skos:broader <http://historyofwork.iisg.nl/resource/033> ;
    skos:definition "Estimates quantities and costs of building materials and labour required for execution of construction projects and prepares bills of quantities."@en ;
    skos:prefLabel "Quantity Surveyor"@en .

<http://historyofwork.iisg.nl/resource/03330> a skos:Concept ;
    skos:broader <http://historyofwork.iisg.nl/resource/033> ;
    skos:definition "Performs technical tasks under direction and supervision of surveyor contributory to execution of surveys and preparation of survey reports."@en ;
    skos:prefLabel "Surveyor's Technician"@en .

<http://historyofwork.iisg.nl/resource/03340> a skos:Concept ;
    skos:broader <http://historyofwork.iisg.nl/resource/033> ;
    skos:definition "Represents building architect on construction site to ensure compliance with design specifications and maintenance of desired standards of materials and workmanship."@en ;
    skos:prefLabel "Clerk of Works"@en .

<http://historyofwork.iisg.nl/resource/03390> a skos:Concept ;
    skos:broader <http://historyofwork.iisg.nl/resource/033> ;
    skos:definition "This group includes civil engineering technicians not elsewhere classified, for example those who visit different construction sites to make measurements, tests and observations to ensure that work done and materials used conform with specifications, to assist contractor in interpretation of working plans and specifications and arrange deviations from specifications to meet regulations governing construction."@en ;
    skos:prefLabel "Other Civil Engineering Technicians"@en .

<http://historyofwork.iisg.nl/resource/03405> a skos:Concept ;
    skos:broader <http://historyofwork.iisg.nl/resource/034> ;
    skos:definition "Performs technical tasks, normally under direction and supervision of electrical engineer, contributory to design, development, construction, installation, maintenance and repair of electrical systems and equipment."@en ;
    skos:prefLabel "Electrical Engineering Technician, General"@en .

<http://historyofwork.iisg.nl/resource/03410> a skos:Concept ;
    skos:broader <http://historyofwork.iisg.nl/resource/034> ;
    skos:definition "Performs technical tasks, normally under direction and supervision of electronics engineer, contributory to design, development, construction, installation, maintenance and repair of electronic devices and equipment."@en ;
    skos:prefLabel "Electronics Engineering Technician, General"@en .

<http://historyofwork.iisg.nl/resource/03420> a skos:Concept ;
    skos:broader <http://historyofwork.iisg.nl/resource/034> ;
    skos:definition "Performs technical tasks, normally under direction and supervision of electrical engineer, contributory to design, development, construction, utilisation, maintenance and repair of high-voltage electrical systems and equipment."@en ;
    skos:prefLabel "Electrical Engineering Technician (High Voltage)"@en .

<http://historyofwork.iisg.nl/resource/03430> a skos:Concept ;
    skos:broader <http://historyofwork.iisg.nl/resource/034> ;
    skos:definition "Performs technical tasks, normally under direction and supervision of telecommunications engineer, contributory to design, development, construction, installation, operation, maintenance and repair of telecommunications systems and equipment."@en ;
    skos:prefLabel "Telecommunications Technician"@en .

<http://historyofwork.iisg.nl/resource/03490> a skos:Concept ;
    skos:broader <http://historyofwork.iisg.nl/resource/034> ;
    skos:definition "This group includes electrical and electronic engineering technicians not elsewhere classified, for example those who perform tasks similar to those of Electrical engineering technician, general (0-34.05) or Electronics engineering technician, general (0-34.10) but specialise in technical tasks contributory to the design, development, construction, maintenance and repair of particular apparatus or products such as electronic calculating and data-processing equipment; radar, radio or television equipment; signalling and automatic control systems; electric traction equipment; electric motors; domestic electrical appliances; or other electrical or electronic apparatus (excluding high-voltage equipment and telecommunications systems)."@en ;
    skos:prefLabel "Other Electrical and Electronics Engineering Technicians"@en .

<http://historyofwork.iisg.nl/resource/03510> a skos:Concept ;
    skos:broader <http://historyofwork.iisg.nl/resource/035> ;
    skos:definition "Performs technical tasks, normally under direction and supervision of mechanical engineer, contributory to design, development, manufacture, construction, installation, efficient operation, maintenance and repair of mechanically functioning plant and equipment."@en ;
    skos:prefLabel "Mechanical Engineering Technician, General"@en .

<http://historyofwork.iisg.nl/resource/03520> a skos:Concept ;
    skos:broader <http://historyofwork.iisg.nl/resource/035> ;
    skos:definition "Performs technical tasks, normally under direction and supervision of mechanical engineer, contributory to design, development, manufacture, installation, maintenance and repair of steam, internal combustion and non-electric motors and engines. Technicians specialising in electric motors are classified in 0-34.90."@en ;
    skos:prefLabel "Mechanical Engineering Technician (Motors and Engines)"@en .

<http://historyofwork.iisg.nl/resource/03530> a skos:Concept ;
    skos:broader <http://historyofwork.iisg.nl/resource/035> ;
    skos:definition "Performs technical tasks, normally under direction and supervision of aeronautical engineer, contributory to design, development, construction, maintenance and repair of aircraft."@en ;
    skos:prefLabel "Aeronautical Engineering Technician"@en .

<http://historyofwork.iisg.nl/resource/03540> a skos:Concept ;
    skos:broader <http://historyofwork.iisg.nl/resource/035> ;
    skos:definition "Performs technical tasks, normally under direction and supervision of automotive engineer, contributory to design, development and manufacture of road vehicles."@en ;
    skos:prefLabel "Automotive Engineering Technician"@en .

<http://historyofwork.iisg.nl/resource/03550> a skos:Concept ;
    skos:broader <http://historyofwork.iisg.nl/resource/035> ;
    skos:definition "Performs technical tasks, normally under direction and supervision of heating, ventilation, and refrigeration engineer, contributory to design, development, manufacture, installation, maintenance and repair of systems and equipment for heating, ventilation and refrigeration."@en ;
    skos:prefLabel "Heating, Ventilation and Refrigeration Engineering Technician"@en .

<http://historyofwork.iisg.nl/resource/03590> a skos:Concept ;
    skos:broader <http://historyofwork.iisg.nl/resource/035> ;
    skos:definition "This group includes mechanical engineering technicians not elsewhere classified, for example those who perform tasks similar to those of Mechanical engineering technician, general (0-35.10) but specialise in technical tasks contributory to the design, production or maintenance of apparatus or products such as plant and equipment for the release, control and utilisation of nuclear energy; ships' hulls and superstructures; precision instruments; cameras and projectors; typewriters, desk calculators, cash registers and ticket machines; duplicating and copying machines; mechanically functioning medical equipment; or special space vehicles and mechanical equipment for space exploration and travel."@en ;
    skos:prefLabel "Other Mechanical Engineering Technicians"@en .

<http://historyofwork.iisg.nl/resource/03610> a skos:Concept ;
    skos:broader <http://historyofwork.iisg.nl/resource/036> ;
    skos:definition "Performs technical tasks, normally under direction and supervision of chemical engineer, contributory to development of processes for the chemical or physical transformation of substances on a commercial scale and to design, construction, operation, maintenance and repair of chemical plant."@en ;
    skos:prefLabel "Chemical Engineering Technical, General"@en .

<http://historyofwork.iisg.nl/resource/03620> a skos:Concept ;
    skos:broader <http://historyofwork.iisg.nl/resource/036> ;
    skos:definition "Performs technical tasks, normally under direction and supervision of chemical engineer (petroleum), contributory to development of processes for refining crude oil and to design, construction, operation, maintenance and repair of refining plant."@en ;
    skos:prefLabel "Chemical Engineering Technician (Petroleum)"@en .

<http://historyofwork.iisg.nl/resource/03690> a skos:Concept ;
    skos:broader <http://historyofwork.iisg.nl/resource/036> ;
    skos:definition "This group includes chemical engineering technicians not elsewhere classified, for example those who perform tasks similar to those of Chemical engineering technician, general (0-36.10) but specialise in technical tasks contributory to development and efficient utilisation of fuels or to design, construction, operation, maintenance and repair of plant for the chemical and physical transformation of matter for the manufacture of a particular type of commodity such as antibiotics, plastics, explosives, rubber or pigments, or of plant for production and distribution of fuel gas for industrial, domestic and other uses."@en ;
    skos:prefLabel "Other Chemical Engineering Technicians"@en .

<http://historyofwork.iisg.nl/resource/03700> a skos:Concept ;
    skos:broader <http://historyofwork.iisg.nl/resource/037> ;
    skos:definition "May perform any (but not all) of the occupational activities described in unit group 0-37."@en ;
    skos:prefLabel "Metallurgical Technician, Specialisation Unknown"@en .

<http://historyofwork.iisg.nl/resource/03720> a skos:Concept ;
    skos:broader <http://historyofwork.iisg.nl/resource/037> ;
    skos:definition "Performs technical tasks, normally under direction and supervision of extractive metallurgist, contributory to development and control of processes for the extraction of metals from their ores."@en ;
    skos:prefLabel "Extractive Metallurgy Technician"@en .

<http://historyofwork.iisg.nl/resource/03730> a skos:Concept ;
    skos:broader <http://historyofwork.iisg.nl/resource/037> ;
    skos:definition "Performs technical tasks, normally under direction and supervision of physical metallurgist, contributory to research into properties of metals and alloys, development of new alloys and technical supervision of metal and alloy manufacture and processing."@en ;
    skos:prefLabel "Physical Metallurgy Technician"@en .

<http://historyofwork.iisg.nl/resource/03790> a skos:Concept ;
    skos:broader <http://historyofwork.iisg.nl/resource/037> ;
    skos:definition "This group includes metallurgical technicians not elsewhere classified, for example those who performtechnical tasks similar to those of Extractive and Physical metallurgy technicians (0-37.20 and 0-37.30) to assist metallurgists specialising in radioactive materials."@en ;
    skos:prefLabel "Other Metallurgical Technicians"@en .

<http://historyofwork.iisg.nl/resource/03810> a skos:Concept ;
    skos:broader <http://historyofwork.iisg.nl/resource/038> ;
    skos:definition "Performs technical tasks, normally under direction and supervision of mining engineer, contributory to the extraction of metallic and solid non-metallic minerals from the earth and their preparation for distribution or processing."@en ;
    skos:prefLabel "Mining Technician, General"@en .

<http://historyofwork.iisg.nl/resource/03820> a skos:Concept ;
    skos:broader <http://historyofwork.iisg.nl/resource/038> ;
    skos:definition "Performs technical tasks, normally under direction and supervision of petroleum and natural gas engineer, contributory to the extraction, storage and transportation of petroleum and natural gas."@en ;
    skos:prefLabel "Petroleum and Natural Gas Extraction Technician"@en .

<http://historyofwork.iisg.nl/resource/03890> a skos:Concept ;
    skos:broader <http://historyofwork.iisg.nl/resource/038> ;
    skos:definition "This group includes mining technicians not elsewhere classified, for example those who perform tasks similar to those of Mining technicians, general (0-38.10) but specialise in technical tasks contributory to the extraction from mines and quarries of a particular solid mineral such as coal, stone, clay, salt, gravel or diamonds; or to extraction of subsurface water or sulphur and other solid minerals by drilling boreholes; or to extraction of tin, gold, diamonds or other solid minerals from alluvial deposits by sluicing and dredging."@en ;
    skos:prefLabel "Other Mining Technicians"@en .

<http://historyofwork.iisg.nl/resource/03920> a skos:Concept ;
    skos:broader <http://historyofwork.iisg.nl/resource/039> ;
    skos:definition "Performs technical tasks, normally under the direction of production methods engineer, to determine for particular products suitable sequences and timings for production operations."@en ;
    skos:prefLabel "Production Engineering Technician"@en .

<http://historyofwork.iisg.nl/resource/03930> a skos:Concept ;
    skos:broader <http://historyofwork.iisg.nl/resource/039> ;
    skos:definition "Performs time and motion studies under direction and supervision of time and motion study engineer."@en ;
    skos:prefLabel "Time and Motion Study Technician"@en .

<http://historyofwork.iisg.nl/resource/03990> a skos:Concept ;
    skos:broader <http://historyofwork.iisg.nl/resource/039> ;
    skos:definition "This group includes engineering technicians not elsewhere classified, for example those who specialise in performing technical tasks contributory to technological development of processes and plant, or technical supervision of processing operations, relating to the manufacture of bricks, pottery and glassware; of food and beverages; textiles; paper; leather or wood products; those assisting safety engineers, agricultural engineers, or traffic planners; and those performing other technical tasks in engineering not performed by workers classified elsewhere."@en ;
    skos:prefLabel "Other Engineering Technicians"@en .

<http://historyofwork.iisg.nl/resource/04120> a skos:Concept ;
    skos:broader <http://historyofwork.iisg.nl/resource/041> ;
    skos:definition "Flies aircraft transporting passengers, mail or freight."@en ;
    skos:prefLabel "Air Transport Pilot"@en .

<http://historyofwork.iisg.nl/resource/04125> a skos:Concept ;
    skos:broader <http://historyofwork.iisg.nl/resource/041> ;
    skos:definition "Flies aircraft for transport of passengers, mail, or freight or for other purposes."@en ;
    skos:prefLabel "Aircraft Pilot (Transport or Other Purposes)"@en .

<http://historyofwork.iisg.nl/resource/04130> a skos:Concept ;
    skos:broader <http://historyofwork.iisg.nl/resource/041> ;
    skos:definition "Pilots aircraft for purposes other than passenger, mail or freight transportation, such as for testing or delivering aircraft, spraying insecticides and fungicides for pest control, aerial surveys, aerial photography, and exhibitions of flying skill."@en ;
    skos:prefLabel "Aircraft Pilot (except Transport)"@en .

<http://historyofwork.iisg.nl/resource/04140> a skos:Concept ;
    skos:broader <http://historyofwork.iisg.nl/resource/041> ;
    skos:definition "Directs course of aircraft in flight according to predetermined flight plan or as directed by pilot-in-command."@en ;
    skos:prefLabel "Flight Navigator"@en .

<http://historyofwork.iisg.nl/resource/04150> a skos:Concept ;
    skos:broader <http://historyofwork.iisg.nl/resource/041> ;
    skos:definition "Makes pre-flight, in-flight and post-flight inspections, carries out adjustments and minor repairs to ensure safe and efficient operation of aircraft and monitors control panel during flight."@en ;
    skos:prefLabel "Flight Engineer"@en .

<http://historyofwork.iisg.nl/resource/04160> a skos:Concept ;
    skos:broader <http://historyofwork.iisg.nl/resource/041> ;
    skos:definition "Teaches trainee pilots to operate the controls of an aircraft and instructs them in aircraft piloting techniques and procedures."@en ;
    skos:prefLabel "Flying Instructor"@en .

<http://historyofwork.iisg.nl/resource/04200> a skos:Concept ;
    skos:broader <http://historyofwork.iisg.nl/resource/042> ;
    skos:definition "May perform any (but not all) of the occupational activities described in unit group 0-42."@en ;
    skos:prefLabel "Ships' Deck Officer or Pilot, Specialisation Unknown"@en .

<http://historyofwork.iisg.nl/resource/04215> a skos:Concept ;
    skos:broader <http://historyofwork.iisg.nl/resource/042> ;
    skos:definition "Takes complete charge of seagoing ship and directs, co-ordinates and supervises shipboard activities."@en ;
    skos:prefLabel "Ship's Master (Sea)"@en .

<http://historyofwork.iisg.nl/resource/04217> a skos:Concept ;
    skos:broader <http://historyofwork.iisg.nl/resource/042> ;
    skos:definition "Takes complete charge of seagoing ship or vessel confined to inland waterways and directs, co-ordinates and supervises shipboard activities."@en ;
    skos:prefLabel "Ship's Master (Sea or Inland Waterways)"@en .

<http://historyofwork.iisg.nl/resource/04220> a skos:Concept ;
    skos:broader <http://historyofwork.iisg.nl/resource/042> ;
    skos:definition "Takes complete charge of vessel confined to inland waterways and directs, co-ordinates and supervises activities on board. Boatman is classified in 9.81.90."@en ;
    skos:prefLabel "Ship's Master (Inland Waterways)"@en .

<http://historyofwork.iisg.nl/resource/04230> a skos:Concept ;
    skos:broader <http://historyofwork.iisg.nl/resource/042> ;
    skos:definition "Plans, supervises and co-ordinates deck and bridge-watch activities on seagoing or inland waterways vessel."@en ;
    skos:prefLabel "Ship's Navigating Officer"@en .

<http://historyofwork.iisg.nl/resource/04240> a skos:Concept ;
    skos:broader <http://historyofwork.iisg.nl/resource/042> ;
    skos:definition "Navigates vessels into and out of ports, in rivers, channels, straits and other waters where special knowledge and skill are required."@en ;
    skos:prefLabel "Ship Pilot"@en .

<http://historyofwork.iisg.nl/resource/04250> a skos:Concept ;
    skos:broader <http://historyofwork.iisg.nl/resource/042> ;
    skos:definition "Directs or arranges on-shore services such as supply of ships' stores and equipment, ship inspections and overhauls, crew replacements and navigational information for shipping company vessels arriving in port. Marine superintendent (technical) is classified in 0-43.30."@en ;
    skos:prefLabel "Marine Superintendent (Deck)"@en .

<http://historyofwork.iisg.nl/resource/04290> a skos:Concept ;
    skos:broader <http://historyofwork.iisg.nl/resource/042> ;
    skos:definition "This group includes ships' deck officers and pilots not elsewhere classified, for example those in charge of seagoing yachts and hovercraft."@en ;
    skos:prefLabel "Other Ships' Deck Officers and Pilots"@en .

<http://historyofwork.iisg.nl/resource/04315> a skos:Concept ;
    skos:broader <http://historyofwork.iisg.nl/resource/043> ;
    skos:definition "Plans, co-ordinates and directs engine-room department aboard ship and supervises subordinate marine engineer officers and engine-room ratings."@en ;
    skos:prefLabel "Ship's Chief Engineer"@en .

<http://historyofwork.iisg.nl/resource/04320> a skos:Concept ;
    skos:broader <http://historyofwork.iisg.nl/resource/043> ;
    skos:definition "Controls, and participates in, the operation, maintenance and repair of engines, electrical motors, boilers, pumps, compressors, heat exchangers, and other machinery and equipment on board ship under the general direction of chief engineer."@en ;
    skos:prefLabel "Marine Engineer Officer"@en .

<http://historyofwork.iisg.nl/resource/04330> a skos:Concept ;
    skos:broader <http://historyofwork.iisg.nl/resource/043> ;
    skos:definition "Directs from shore station the maintenance programmes for machinery and equipment on board company's ships, directs or authorises repairs in port and directs replacement programme for shipboard machinery."@en ;
    skos:prefLabel "Marine Superintendent (Technical)"@en .

<http://historyofwork.iisg.nl/resource/05110> a skos:Concept ;
    skos:broader <http://historyofwork.iisg.nl/resource/051> ;
    skos:definition "Conducts research into all forms of life to increase scientific knowledge and develops practical applications in fields such as medicine and agriculture."@en ;
    skos:prefLabel "Biologist, General"@en .

<http://historyofwork.iisg.nl/resource/05120> a skos:Concept ;
    skos:broader <http://historyofwork.iisg.nl/resource/051> ;
    skos:definition "Conducts research into all forms of plant life to increase scientific knowledge and develop practical applications in fields such as agriculture and forestry."@en ;
    skos:prefLabel "Botanist"@en .

<http://historyofwork.iisg.nl/resource/05130> a skos:Concept ;
    skos:broader <http://historyofwork.iisg.nl/resource/051> ;
    skos:definition "Conducts research into all forms of animal life to increase scientific knowledge and develop practical applications in fields such as agriculture and medicine."@en ;
    skos:prefLabel "Zoologist"@en .

<http://historyofwork.iisg.nl/resource/05190> a skos:Concept ;
    skos:broader <http://historyofwork.iisg.nl/resource/051> ;
    skos:definition "This group includes biologists, zoologists and related scientists not elsewhere classified, for example those who specialise in marine and freshwater life."@en ;
    skos:prefLabel "Other Biologists, Zoologists and Related Scientists"@en .

<http://historyofwork.iisg.nl/resource/05220> a skos:Concept ;
    skos:broader <http://historyofwork.iisg.nl/resource/052> ;
    skos:definition "Conducts research into the form, structure and other anatomical characteristics of humans and animals to increase scientific knowledge and develop practical applications in medical and related fields."@en ;
    skos:prefLabel "Anatomist"@en .

<http://historyofwork.iisg.nl/resource/05230> a skos:Concept ;
    skos:broader <http://historyofwork.iisg.nl/resource/052> ;
    skos:definition "Conducts research into chemical composition and processes of living organisms to increase scientific knowledge and develop industrial, medical and other practical applications."@en ;
    skos:prefLabel "Biochemist"@en .

<http://historyofwork.iisg.nl/resource/05240> a skos:Concept ;
    skos:broader <http://historyofwork.iisg.nl/resource/052> ;
    skos:definition "Conducts research into biological functions and activities of human organism under normal and abnormal conditions to increase scientific knowledge and develop practical applications in medical and related fields."@en ;
    skos:prefLabel "Physiologist"@en .

<http://historyofwork.iisg.nl/resource/05250> a skos:Concept ;
    skos:broader <http://historyofwork.iisg.nl/resource/052> ;
    skos:definition "Conducts research into nature and characteristics of bacteria and other micro-organisms to increase scientific knowledge and develop industrial, medical and other practical applications."@en ;
    skos:prefLabel "Bacteriologist"@en .

<http://historyofwork.iisg.nl/resource/05260> a skos:Concept ;
    skos:broader <http://historyofwork.iisg.nl/resource/052> ;
    skos:definition "Conducts research into nature, causes and development of human diseases and disorders."@en ;
    skos:prefLabel "Medical Pathologist"@en .

<http://historyofwork.iisg.nl/resource/05265> a skos:Concept ;
    skos:broader <http://historyofwork.iisg.nl/resource/052> ;
    skos:definition "Conducts research into nature, causes and development of animal diseases and disorders."@en ;
    skos:prefLabel "Veterinary Pathologist"@en .

<http://historyofwork.iisg.nl/resource/05270> a skos:Concept ;
    skos:broader <http://historyofwork.iisg.nl/resource/052> ;
    skos:definition "Conducts research into effects of drugs and other substances on organs, tissues and life processes of humans and animals and develops new and improved medicinal drugs."@en ;
    skos:prefLabel "Pharmacologist"@en .

<http://historyofwork.iisg.nl/resource/05280> a skos:Concept ;
    skos:broader <http://historyofwork.iisg.nl/resource/052> ;
    skos:definition "Conducts research into animal genetics, advanced animal husbandry methods and related matters and applies scientific knowledge to develop improved strains, improved methods of raising animals and higher yields of animal products."@en ;
    skos:prefLabel "Animal Scientist"@en .

<http://historyofwork.iisg.nl/resource/05290> a skos:Concept ;
    skos:broader <http://historyofwork.iisg.nl/resource/052> ;
    skos:definition "This group includes bacteriologists, pharmacologists and related scientists not elsewhere classified, for example those conducting research in the field of biophysics, relating to such problems as dynamics of seeing and hearing, transmission of electrical impulses along nerves and muscles, effects of light and other radiation on body cells, and developing practical applications for medical or other purposes."@en ;
    skos:prefLabel "Other Bacteriologists, Pharmacologists and Related Scientists"@en .

<http://historyofwork.iisg.nl/resource/05320> a skos:Concept ;
    skos:broader <http://historyofwork.iisg.nl/resource/053> ;
    skos:definition "Conducts research into field crops and grasses and develops new and improved production methods."@en ;
    skos:prefLabel "Agronomist"@en .

<http://historyofwork.iisg.nl/resource/05330> a skos:Concept ;
    skos:broader <http://historyofwork.iisg.nl/resource/053> ;
    skos:definition "Conducts research into horticultural crops and develops new and improved production methods."@en ;
    skos:prefLabel "Horticulturist"@en .

<http://historyofwork.iisg.nl/resource/05340> a skos:Concept ;
    skos:broader <http://historyofwork.iisg.nl/resource/053> ;
    skos:definition "Conducts research into, and develops methods of, tree propagation and culture and plans and directs afforestation, care and exploitation of forest stands."@en ;
    skos:prefLabel "Silviculturist"@en .

<http://historyofwork.iisg.nl/resource/05350> a skos:Concept ;
    skos:broader <http://historyofwork.iisg.nl/resource/053> ;
    skos:definition "Conducts research into characteristics, use capabilities and productivity of soils and applies findings to development of improved agricultural, horticultural and forestry practices."@en ;
    skos:prefLabel "Soil Scientist"@en .

<http://historyofwork.iisg.nl/resource/05360> a skos:Concept ;
    skos:broader <http://historyofwork.iisg.nl/resource/053> ;
    skos:definition "Advises farmers on farming methods and problems."@en ;
    skos:prefLabel "Farming Adviser"@en .

<http://historyofwork.iisg.nl/resource/05390> a skos:Concept ;
    skos:broader <http://historyofwork.iisg.nl/resource/053> ;
    skos:definition "This group includes agronomists and related scientists not elsewhere classified, for example those who investigate conditions and problems, make recommendations and develop improved methods relating to conservation of wild life reserves or economic exploitation of grazing lands."@en ;
    skos:prefLabel "Other Agronomists and Related Scientists"@en .

<http://historyofwork.iisg.nl/resource/05400> a skos:Concept ;
    skos:broader <http://historyofwork.iisg.nl/resource/054> ;
    skos:definition "May perform any (but not all) of the occupational activities described in unit group 0-54."@en ;
    skos:prefLabel "Life Science Technician, Specialisation Unknown"@en .

<http://historyofwork.iisg.nl/resource/05420> a skos:Concept ;
    skos:broader <http://historyofwork.iisg.nl/resource/054> ;
    skos:definition "Performs technical tasks, normally under direction and supervision of biological scientist, contributory to biological experiments, tests and analyses to increase scientific knowledge and develop industrial, public health, agricultural and other practical applications."@en ;
    skos:prefLabel "Biological Technician"@en .

<http://historyofwork.iisg.nl/resource/05430> a skos:Concept ;
    skos:broader <http://historyofwork.iisg.nl/resource/054> ;
    skos:definition "Performs technical tasks, normally under direction and supervision of medical scientist, contributory to experiments, tests and analyses for the diagnosis, treatment and prevention of sickness and disease."@en ;
    skos:prefLabel "Medical Science Technician"@en .

<http://historyofwork.iisg.nl/resource/05490> a skos:Concept ;
    skos:broader <http://historyofwork.iisg.nl/resource/054> ;
    skos:definition "This group includes life sciences technicians not elsewhere classified, for example those who specialise in performing technical tasks in connection with the collection, treatment, storage and distribution of semen for artificial breeding of farm animals; performing technical tasks to assist agronomists, horticulturists and silviculturists; or analysing samples of seeds for quality, purity and germination rating."@en ;
    skos:prefLabel "Other Life Sciences Technicians"@en .

<http://historyofwork.iisg.nl/resource/06100> a skos:Concept ;
    skos:broader <http://historyofwork.iisg.nl/resource/061> ;
    skos:definition "May perform any (but not all) of the occupational activities described in unit group 0-61."@en ;
    skos:prefLabel "Medical Doctor, Specialisation Unknown"@en .

<http://historyofwork.iisg.nl/resource/06105> a skos:Concept ;
    skos:broader <http://historyofwork.iisg.nl/resource/061> ;
    skos:definition "Conducts medical examinations, makes diagnoses, prescribes medicines, and gives other forms of treatment for various kinds of diseases, disorders and injuries of the human body; applies preventive medicine techniques to prevent diseases and promote good health."@en ;
    skos:prefLabel "General Physician"@en .

<http://historyofwork.iisg.nl/resource/06110> a skos:Concept ;
    skos:broader <http://historyofwork.iisg.nl/resource/061> ;
    skos:definition "Performs various kinds of surgical operations in the treatment of injuries, diseases and disorders of the human body."@en ;
    skos:prefLabel "General Surgeon"@en .

<http://historyofwork.iisg.nl/resource/06120> a skos:Concept ;
    skos:broader <http://historyofwork.iisg.nl/resource/061> ;
    skos:definition "Specialises in giving medical treatment and advice for particular types of diseases, disorders and injuries of the human body."@en ;
    skos:prefLabel "Specialised Physician"@en .

<http://historyofwork.iisg.nl/resource/06130> a skos:Concept ;
    skos:broader <http://historyofwork.iisg.nl/resource/061> ;
    skos:definition "Specialises in giving surgical treatment and advice for particular types of diseases and disorders of the human body."@en ;
    skos:prefLabel "Specialised Surgeon"@en .

<http://historyofwork.iisg.nl/resource/06140> a skos:Concept ;
    skos:broader <http://historyofwork.iisg.nl/resource/061> ;
    skos:definition "Exercises controls and supervision to implement or enforce public health laws and regulations for safeguarding and promoting the health of a community."@en ;
    skos:prefLabel "Public Health Physician"@en .

<http://historyofwork.iisg.nl/resource/06190> a skos:Concept ;
    skos:broader <http://historyofwork.iisg.nl/resource/061> ;
    skos:definition "This group includes medical doctors not elsewhere classified, for example those mainly employed in conducting medical examinations in schools, workplaces or elsewhere; those mainly employed in giving medical advice, for instance in connection with life or other insurance plans, social security funds, medical aspects of occupational risks, or otherwise."@en ;
    skos:prefLabel "Other Medical Doctors"@en .

<http://historyofwork.iisg.nl/resource/06210> a skos:Concept ;
    skos:broader <http://historyofwork.iisg.nl/resource/062> ;
    skos:definition "Performs to a limited extent the tasks of General physician (0-61.05) within a public health service or institution, more particularly as regards common diseases of the region, either independently or under the general direction of a fully qualified physician. The workers in this group have not had the full training of General physician (0-61.05)."@en ;
    skos:prefLabel "Medical Assistant"@en .

<http://historyofwork.iisg.nl/resource/06310> a skos:Concept ;
    skos:broader <http://historyofwork.iisg.nl/resource/063> ;
    skos:definition "Performs diagnostic, preventive and curative services for dental or oral diseases and disorders."@en ;
    skos:prefLabel "Dentist, General"@en .

<http://historyofwork.iisg.nl/resource/06320> a skos:Concept ;
    skos:broader <http://historyofwork.iisg.nl/resource/063> ;
    skos:definition "Specialises in giving surgical, medical and other forms of treatment for particular types of dental and oral diseases and disorders."@en ;
    skos:prefLabel "Specialised Dentist"@en .

<http://historyofwork.iisg.nl/resource/06330> a skos:Concept ;
    skos:broader <http://historyofwork.iisg.nl/resource/063> ;
    skos:definition "Plans and directs public action to improve oral health and to control and improve standards of dental care and treatment of oral disorders."@en ;
    skos:prefLabel "Public Health Dentist"@en .

<http://historyofwork.iisg.nl/resource/06420> a skos:Concept ;
    skos:broader <http://historyofwork.iisg.nl/resource/064> ;
    skos:definition "Carries out, but only to a limited extent, diagnostic, preventive and curative tasks in dentistry to assist dentists, or independently. The workers in this group have not had the full training of Dentists (0-63), and may be designated Practical dentist, Unregistered dentist or Dental auxiliary."@en ;
    skos:prefLabel "Dental Assistant"@en .

<http://historyofwork.iisg.nl/resource/06430> a skos:Concept ;
    skos:broader <http://historyofwork.iisg.nl/resource/064> ;
    skos:definition "Performs limited diagnostic, preventive and curative duties in dentistry for pre-school and schoolchildren under the direction and control of a dentist."@en ;
    skos:prefLabel "School Dental Assistant"@en .

<http://historyofwork.iisg.nl/resource/06440> a skos:Concept ;
    skos:broader <http://historyofwork.iisg.nl/resource/064> ;
    skos:definition "Carries out dental prophylactic treatments and instructs groups and individuals in care of teeth and mouth."@en ;
    skos:prefLabel "Dental Hygienist"@en .

<http://historyofwork.iisg.nl/resource/06510> a skos:Concept ;
    skos:broader <http://historyofwork.iisg.nl/resource/065> ;
    skos:definition "Diagnoses and gives or prescribes medical and surgical treatment of diseases, injuries or other medical conditions of animals and deals with other aspects of animal health."@en ;
    skos:prefLabel "Veterinarian, General"@en .

<http://historyofwork.iisg.nl/resource/06520> a skos:Concept ;
    skos:broader <http://historyofwork.iisg.nl/resource/065> ;
    skos:definition "Exercises surveillance of quality, purity and safety of food of animal origin intended for human consumption and investigates and controls animal diseases hazardous to man."@en ;
    skos:prefLabel "Public Health Veterinarian"@en .

<http://historyofwork.iisg.nl/resource/06590> a skos:Concept ;
    skos:broader <http://historyofwork.iisg.nl/resource/065> ;
    skos:definition "This group includes veterinarians not elsewhere classified, for example those controlling import and export of animals and animal products; controlling drugs and vaccines used in veterinary practise; advising on the breeding, transport, care and health problems of laboratory animals; advising on and assisting in epidemiological and other surveillance of zoonoses; collaborating in the preparation of animals for space exploration experiments."@en ;
    skos:prefLabel "Other Veterinarians"@en .

<http://historyofwork.iisg.nl/resource/06610> a skos:Concept ;
    skos:broader <http://historyofwork.iisg.nl/resource/066> ;
    skos:definition "Carries out, but only to a limited extent, diagnostic, preventive and curative veterinary duties as described under Veterinarian, general (0-65.10), more particularly as regards common diseases and disorders of animals, either independently or under the general direction of fully qualified veterinarian. The workers in this group have not had the full training of Veterinarians (0-65)."@en ;
    skos:prefLabel "Veterinary Assistant"@en .

<http://historyofwork.iisg.nl/resource/06710> a skos:Concept ;
    skos:broader <http://historyofwork.iisg.nl/resource/067> ;
    skos:definition "Makes and dispenses medicaments and related preparations according to prescriptions or formulae."@en ;
    skos:prefLabel "Pharmacist"@en .

<http://historyofwork.iisg.nl/resource/06810> a skos:Concept ;
    skos:broader <http://historyofwork.iisg.nl/resource/068> ;
    skos:definition "Assists in a pharmacy, hospital or dispensary to make and dispense medicaments, under the direction of a pharmacist."@en ;
    skos:prefLabel "Pharmaceutical Assistant"@en .

<http://historyofwork.iisg.nl/resource/06910> a skos:Concept ;
    skos:broader <http://historyofwork.iisg.nl/resource/069> ;
    skos:definition "Plans and supervises the preparation of therapeutic or other diets for individuals or for groups in hospitals, institutions and other establishments and for workers in particular sectors; gives instruction in selection and proper preparation of food according to dietetic principles; performs duties related to nutrition programmes."@en ;
    skos:prefLabel "Dietitian, General"@en .

<http://historyofwork.iisg.nl/resource/06920> a skos:Concept ;
    skos:broader <http://historyofwork.iisg.nl/resource/069> ;
    skos:definition "Appraises various factors related to nutrition and food problems in the community and plans and executes nutrition elements of health programmes."@en ;
    skos:prefLabel "Public Health Nutritionist"@en .

<http://historyofwork.iisg.nl/resource/06990> a skos:Concept ;
    skos:broader <http://historyofwork.iisg.nl/resource/069> ;
    skos:definition "This group includes dietitians and public health nutritionists not elsewhere classified, for example those acting as consultants to food processing and distributing firms or to manufacturers of food-processing equipment."@en ;
    skos:prefLabel "Other Dietitians and Public Health Nutritionists"@en .

<http://historyofwork.iisg.nl/resource/07110> a skos:Concept ;
    skos:broader <http://historyofwork.iisg.nl/resource/071> ;
    skos:definition "Provides professional nursing services and advice in hospitals, clinics or other establishments which provide medical care and treatment."@en ;
    skos:prefLabel "Professional Nurse, General"@en .

<http://historyofwork.iisg.nl/resource/07120> a skos:Concept ;
    skos:broader <http://historyofwork.iisg.nl/resource/071> ;
    skos:definition "Provides specialised professional nursing services in a medical establishment or elsewhere."@en ;
    skos:prefLabel "Specialised Nurse"@en .

<http://historyofwork.iisg.nl/resource/07130> a skos:Concept ;
    skos:broader <http://historyofwork.iisg.nl/resource/071> ;
    skos:definition "Provides, within a community health service, professional nursing care and advice in private homes, schools, maternal and child health centres and nurseries; performs other nursing tasks associated with the provision of community health services."@en ;
    skos:prefLabel "Public Health Nurse"@en .

<http://historyofwork.iisg.nl/resource/07140> a skos:Concept ;
    skos:broader <http://historyofwork.iisg.nl/resource/071> ;
    skos:definition "Provides professional nursing services and health information for employees in workplaces."@en ;
    skos:prefLabel "Occupational Health Nurse"@en .

<http://historyofwork.iisg.nl/resource/07190> a skos:Concept ;
    skos:broader <http://historyofwork.iisg.nl/resource/071> ;
    skos:definition "This group includes professional nurses not elsewhere classified, for example those specialising in provision of consultant services to industrial and other organisations; or in giving private general nursing care to patients in their homes."@en ;
    skos:prefLabel "Other Professional Nurses"@en .

<http://historyofwork.iisg.nl/resource/07210> a skos:Concept ;
    skos:broader <http://historyofwork.iisg.nl/resource/072> ;
    skos:definition "Provides simple nursing services to patients, generally under the supervision of a physician or professional nurse. Nursing aid is classified in 5-99.40."@en ;
    skos:prefLabel "Auxiliary Nurse"@en .

<http://historyofwork.iisg.nl/resource/07310> a skos:Concept ;
    skos:broader <http://historyofwork.iisg.nl/resource/073> ;
    skos:definition "Gives professional care and advice to women to aid them during pregnancy, childbirth and the postnatal period. A professional nurse specialising in obstetrics is classified as Specialised nurse (0-71.20)."@en ;
    skos:prefLabel "Professional Midwife"@en .

<http://historyofwork.iisg.nl/resource/07410> a skos:Concept ;
    skos:broader <http://historyofwork.iisg.nl/resource/074> ;
    skos:definition "Provides practical care and assistance to women, usually in private homes, to aid them during pregnancy, childbirth and the postnatal period; takes care of the new-born infant. The workers classified in this group do not have the full training and theoretical knowledge of Professional midwife (0-73.10)."@en ;
    skos:prefLabel "Auxiliary Midwife"@en .

<http://historyofwork.iisg.nl/resource/07520> a skos:Concept ;
    skos:broader <http://historyofwork.iisg.nl/resource/075> ;
    skos:definition "Examines eyes and prescribes spectacles or treatment not involving the use of medicines, surgery or drugs, to conserve or improve vision."@en ;
    skos:prefLabel "Optometrist"@en .

<http://historyofwork.iisg.nl/resource/07530> a skos:Concept ;
    skos:broader <http://historyofwork.iisg.nl/resource/075> ;
    skos:definition "Assists customer in choice of frames, selects the lenses prescribed, fits lenses in frames and fits frames to customer, or fits contact lenses according to prescription."@en ;
    skos:prefLabel "Dispensing Optician"@en .

<http://historyofwork.iisg.nl/resource/07620> a skos:Concept ;
    skos:broader <http://historyofwork.iisg.nl/resource/076> ;
    skos:definition "Treats sprains, healing fractures, paralysis, circulatory and nervous disorders by physical means, usually as prescribed by a physician."@en ;
    skos:prefLabel "Physiotherapist"@en .

<http://historyofwork.iisg.nl/resource/07630> a skos:Concept ;
    skos:broader <http://historyofwork.iisg.nl/resource/076> ;
    skos:definition "Participates in planned medically oriented vocational, educational or recreational activities designed to rehabilitate physically or mentally disabled persons."@en ;
    skos:prefLabel "Occupational Therapist"@en .

<http://historyofwork.iisg.nl/resource/07640> a skos:Concept ;
    skos:broader <http://historyofwork.iisg.nl/resource/076> ;
    skos:definition "Massages clients or patients to improve circulation, soothe or stimulate nerves, facilitate elimination of waste matter, stretch contracted tendons and produce other therapeutic effects."@en ;
    skos:prefLabel "Masseur"@en .

<http://historyofwork.iisg.nl/resource/07710> a skos:Concept ;
    skos:broader <http://historyofwork.iisg.nl/resource/077> ;
    skos:definition "Operates X-ray equipment to make radiographs for medical diagnostic purposes or to give therapeutic treatment."@en ;
    skos:prefLabel "Medical X-Ray Technician"@en .

<http://historyofwork.iisg.nl/resource/07920> a skos:Concept ;
    skos:broader <http://historyofwork.iisg.nl/resource/079> ;
    skos:definition "Diagnoses and treats, mainly by manipulative methods, disorders of bones, muscles, blood vessels and other tissues of the human body."@en ;
    skos:prefLabel "Osteopath"@en .

<http://historyofwork.iisg.nl/resource/07930> a skos:Concept ;
    skos:broader <http://historyofwork.iisg.nl/resource/079> ;
    skos:definition "Relieves illness believed due to pressure upon nervous system at the spine by adjusting joints of the spine."@en ;
    skos:prefLabel "Chiropractor"@en .

<http://historyofwork.iisg.nl/resource/07940> a skos:Concept ;
    skos:broader <http://historyofwork.iisg.nl/resource/079> ;
    skos:definition "Inspects the environment, promotes measures to restore or improve sanitary conditions and supervises their implementation.Sanitary engineers are classified in 0-22.50."@en ;
    skos:prefLabel "Sanitarian"@en .

<http://historyofwork.iisg.nl/resource/07950> a skos:Concept ;
    skos:broader <http://historyofwork.iisg.nl/resource/079> ;
    skos:definition "Writes specifications for and fits artificial limbs, braces and other appliances for body deformities and disorders following prescription of physician."@en ;
    skos:prefLabel "Orthopaedic Technician"@en .

<http://historyofwork.iisg.nl/resource/07990> a skos:Concept ;
    skos:broader <http://historyofwork.iisg.nl/resource/079> ;
    skos:definition "This group includes medical, dental, veterinary and related workers not elsewhere classified, for example those treating sickness through the application of various herbs and medicinal plants; those treating patients with a system of physical culture and drugless treatment of disease by methods aimed to stimulate or assist nature; those treating body ailments and nervous disorders through mental influence and suggestion; those who treat physical ailments by means of therapeutic baths and other treatments; those carrying out minor surgical procedures connected, for example, with ailments of the human foot; those diagnosing and treating minor ailments of the human foot such as corns, callouses, deformed toenails, flat feet and other disorders and advising patients on further treatment, proper foot care and suitable footwear."@en ;
    skos:prefLabel "Other Medical, Dental, Veterinary and Related Workers"@en .

<http://historyofwork.iisg.nl/resource/08110> a skos:Concept ;
    skos:broader <http://historyofwork.iisg.nl/resource/081> ;
    skos:definition "Conducts research to develop new and improved statistical methods, advises on practical applications of statistical methods, plans and conducts statistical surveys, and organises, analyses and interprets statistical data."@en ;
    skos:prefLabel "Statistician, General"@en .

<http://historyofwork.iisg.nl/resource/08120> a skos:Concept ;
    skos:broader <http://historyofwork.iisg.nl/resource/081> ;
    skos:definition "Conducts research into mathematical basis of science of statistics, develops new and improved statistical methodology and advises on practical applications of statistical methods and techniques."@en ;
    skos:prefLabel "Mathematical Statistician"@en .

<http://historyofwork.iisg.nl/resource/08130> a skos:Concept ;
    skos:broader <http://historyofwork.iisg.nl/resource/081> ;
    skos:definition "Plans and conducts statistical surveys, evaluates, organises, analyses and interprets statistical data and prepares reports."@en ;
    skos:prefLabel "Statistician (Applied Statistics)"@en .

<http://historyofwork.iisg.nl/resource/08220> a skos:Concept ;
    skos:broader <http://historyofwork.iisg.nl/resource/082> ;
    skos:definition "Conducts research in fundamental mathematics to advance mathematical knowledge and develop and improve mathematical techniques."@en ;
    skos:prefLabel "Mathematician (Pure Mathematics)"@en .

<http://historyofwork.iisg.nl/resource/08230> a skos:Concept ;
    skos:broader <http://historyofwork.iisg.nl/resource/082> ;
    skos:definition "Advises on practical applications of mathematical principles and techniques and applies them to solution of problems in scientific research, engineering, management and other activities. Workers specialising in operations-research analysis are classified in 0-82.40."@en ;
    skos:prefLabel "Mathematician (Applied Mathematics)"@en .

<http://historyofwork.iisg.nl/resource/08240> a skos:Concept ;
    skos:broader <http://historyofwork.iisg.nl/resource/082> ;
    skos:definition "Conducts logical analyses of management problems and formulates mathematical model of each problem for programming and solution by computer."@en ;
    skos:prefLabel "Operations-Research Analyst"@en .

<http://historyofwork.iisg.nl/resource/08250> a skos:Concept ;
    skos:broader <http://historyofwork.iisg.nl/resource/082> ;
    skos:definition "Applies knowledge of mathematics, statistics and financial affairs to design and operation of pension schemes and life, health, social and casualty insurance systems."@en ;
    skos:prefLabel "Actuary"@en .

<http://historyofwork.iisg.nl/resource/08310> a skos:Concept ;
    skos:broader <http://historyofwork.iisg.nl/resource/083> ;
    skos:definition "Analyses data-processing needs and problems of client or employer, advises on feasibility of automatic data-processing and develops appropriate systems and procedures. Operations-research analyst is classified in 0-82.40."@en ;
    skos:prefLabel "Systems Analyst"@en .

<http://historyofwork.iisg.nl/resource/08420> a skos:Concept ;
    skos:broader <http://historyofwork.iisg.nl/resource/084> ;
    skos:definition "Prepares programmes to control automatic processing of data by computer."@en ;
    skos:prefLabel "Computer Programmer"@en .

<http://historyofwork.iisg.nl/resource/08490> a skos:Concept ;
    skos:broader <http://historyofwork.iisg.nl/resource/084> ;
    skos:definition "This group includes statistical and mathematical technicians not elsewhere classified, for example those who carry out, normally under the direction and supervision of statisticians, mathematicians and actuaries, technical tasks contributory to research in statistical, mathematical and actuarial sciences, to analysis, mathematical formulation and solution of problems, and to other practical applications of statistical, mathematical and actuarial methods and techniques."@en ;
    skos:prefLabel "Other Statistical and Mathematical Technicians"@en .

<http://historyofwork.iisg.nl/resource/09010> a skos:Concept ;
    skos:broader <http://historyofwork.iisg.nl/resource/090> ;
    skos:definition "Conducts research and applies the principles and theories of economics to formulate solutions to economic problems."@en ;
    skos:prefLabel "Economist, General"@en .

<http://historyofwork.iisg.nl/resource/09020> a skos:Concept ;
    skos:broader <http://historyofwork.iisg.nl/resource/090> ;
    skos:definition "Conducts research and advises on economic problems in a particular branch of economics."@en ;
    skos:prefLabel "Economist, Specialised"@en .

<http://historyofwork.iisg.nl/resource/09030> a skos:Concept ;
    skos:altLabel " aux malades",
        " g",
        " l'Alcan",
        " l'Alcan, etc.",
        " l'asile",
        " l'h",
        " l'hospice",
        " la base transit air 144)",
        " la poudrerie d'angoul",
        " la radiodiffusion t",
        " sudaviation",
        "(e) aux malades",
        "1ste styrmand seilskib",
        "2den styrmand",
        "2den styrmand seilskib",
        "Abacero",
        "Accoucheuse",
        "Ackusch",
        "Actuaire",
        "Aeronaut",
        "Agronom",
        "Agronome",
        "Agronome-aviculteur",
        "Agronome-g",
        "Agronomstuderande",
        "Aide arpenteur",
        "Aide chimiste",
        "Aide de laboratoire",
        "Aide infirmi",
        "Aide laborantine",
        "Aide pharmacien",
        "Aide-garde-malade",
        "Aide-infirmier",
        "Aide-technicien",
        "Aide-technicienne ",
        "Aktuarie",
        "Albeitar",
        "Amanuensis",
        "Amtsagronom",
        "Amtsdyrl",
        "Analyseur du temps",
        "Analyst",
        "Analyste",
        "Analyste ",
        "Analyste en m",
        "Ancienne sage-femme",
        "Anden styrmand",
        "Andre lantm",
        "Andre styrman",
        "Animateur",
        "Apothecer",
        "Apotheker",
        "Apothekerl",
        "Apothiquaire",
        "Architect",
        "Architecte",
        "Architecte communal",
        "Architecte communal/ville",
        "Architecte de ville",
        "Architecte diplom",
        "Architecte et Peintre",
        "Architecte v",
        "Architecte-industriel",
        "Architekt",
        "Arkitekt",
        "Arpenteur",
        "Arpenteur g",
        "Arpenteur-g",
        "Arpenteur-ing",
        "Arpenteur-n",
        "Artiste v",
        "Arts",
        "Arzt",
        "Aspirant pilote",
        "Assistant v",
        "Assistant(e)-technicien(ne)",
        "Assistant-arpenteur",
        "Assistant-chimiste",
        "Assistant-chimiste a Arvida",
        "Assistant-ing",
        "Assistant-technicien",
        "Assistante-technicienne",
        "Auixliar Enfermer",
        "Auktuarie",
        "Auxiliar Hospital",
        "Aviateur",
        "Aviateur au camp de Bagotville",
        "Aviateur-chef",
        "Avvittringslantm",
        "B",
        "Badare",
        "Badareelev",
        "Bademutter",
        "Badf",
        "Badm",
        "Baningenj",
        "Barberare",
        "Barberarebitr",
        "Barberareelev",
        "Barberareges",
        "Barberarel",
        "Barbererska",
        "Barge captain",
        "Barnmorska",
        "Barnmorskeelev",
        "Barnsjuksk",
        "Barnv",
        "Bauaufseher",
        "Bauf",
        "Bauinspektor",
        "Bautechniker",
        "Bauzeichner",
        "Bauzeichnerin",
        "Bergingeni",
        "Bergsingenj",
        "Betriebswirt",
        "Biochimiste",
        "Biologiste",
        "Bitr",
        "Botaniste",
        "Bouwkundige",
        "Brancardier",
        "Bridgebuilder",
        "Brillenh",
        "Byggnadsingenj",
        "Byggnadsritare",
        "Byggnadstekniker",
        "Byr",
        "Callista",
        "Candidaat-chemicus",
        "Candidat en m",
        "Candidat en pharmacie",
        "Capit",
        "Capitaine",
        "Capitaine au long cours",
        "Capitaine de chaloupe",
        "Castrador",
        "Cha",
        "Chauffagiste",
        "Chef m",
        "Chefarzt. DR.",
        "Chemicus",
        "Chemiker",
        "Chemist",
        "Chimiste",
        "Chiropraticien",
        "Chirurg",
        "Chirurgien",
        "Chirurgien dentiste",
        "Chirurgien docteur",
        "Chirurgien m",
        "Chirurgien-accoucheur",
        "Chirurgien-dentiste",
        "Chirurgijn",
        "Chronom",
        "Cirujano",
        "Cirujano romancista",
        "Cirujia",
        "Cirurgia",
        "Civil engineer",
        "Civilingenj",
        "Civiltopograf",
        "Clerk of works",
        "Commis herboriste",
        "Constructeur",
        "Contramestre de navio",
        "D",
        "Dampskibslods",
        "Dentist",
        "Dentista",
        "Dentiste",
        "Dentiste ambulant",
        "Dentistelev",
        "Dentistin",
        "Dermatologiste",
        "Dermatologue",
        "Dessinateur",
        "Dessinateur architecte",
        "Dessinateur g",
        "Dessinateur industriel",
        "Dessinateur lithographe",
        "Dessinateur paysagiste",
        "Dessinateur-m",
        "Dessinatrice",
        "Di",
        "Dierenarts",
        "Diplomingenieur",
        "Diplomingenj",
        "Distriktslantm",
        "Docteur en m",
        "Doctor",
        "Doctor in de genees- heel en",
        "Doctoresse",
        "Dokter",
        "Doktor",
        "Drogist",
        "Dyrl",
        "E.f",
        "E.kronolots",
        "E.lantm",
        "E.lots",
        "E.mariningenj",
        "E.o.ritare",
        "E.riterska",
        "E.styrman",
        "Economiste",
        "Eerste luitenant vliegenier",
        "El",
        "Electrical engineer",
        "Electricien-ing",
        "Electro-technicus",
        "Elektricitetsingenj",
        "Elektricitetstekniker",
        "Elektroingenieur",
        "Engenheiro Agr",
        "Engenheiro Silvicultor",
        "Engenheiro de minas",
        "Entomolog",
        "Epedemisjuksk",
        "Estudiant Medecina",
        "Estudiante Medicina",
        "Etudiant en m",
        "Etudiant en pharmacie",
        "Etudiant en physioth",
        "Etudiant/",
        "Etudiante en dentisterie",
        "Etudiante garde-malade",
        "Examinerad barnmorska",
        "Explorateur",
        "Extra barnmorska",
        "F",
        "F.d.agronom",
        "F.d.aktuarie",
        "F.d.bergsingenj",
        "F.d.byggnadsingenj",
        "F.d.civilingenj",
        "F.d.dentist",
        "F.d.f",
        "F.d.hemsk",
        "F.d.ingenj",
        "F.d.kartarbetare",
        "F.d.kartf",
        "F.d.kartograf",
        "F.d.kartriterska",
        "F.d.kemist",
        "F.d.kofferdikonstapel",
        "F.d.kommissionslantm",
        "F.d.kronolots",
        "F.d.laborator",
        "F.d.lantm",
        "F.d.maskiningenj",
        "F.d.privatsjuksk",
        "F.d.ritare",
        "F.d.riterska",
        "F.d.sjukgymnast",
        "F.d.skeppsbyggm",
        "F.d.stadsgeolog",
        "F.d.tandtekniker",
        "Feldmesser",
        "Feldscher",
        "Fleischbeschauer",
        "Fleischbeschauter",
        "Flugzeugf",
        "Flygare",
        "Flygingenj",
        "Formerly ladies' nurse",
        "Fotokemigraf",
        "Fotokemist",
        "Fr",
        "Fyringenj",
        "G",
        "Gar",
        "Garde-malade",
        "Garde-malade auxiliaire",
        "Gasverksingenj",
        "Ge",
        "Gemeente architect",
        "Geneesheer",
        "Geodet",
        "Gepensioneerd kapitein",
        "Germana Hospital",
        "Gruvingenj",
        "Gruvs",
        "H",
        "Handelskemist",
        "Hebamme",
        "Hebammenschwester",
        "Hebarzt",
        "Heel- en verloskundige",
        "Heel- en vroedmeester",
        "Herbolari",
        "Herbolario",
        "Herboriste",
        "Hermana Hospital",
        "Hochbautechniker",
        "Hongreur",
        "Hulpapotheker",
        "Hydrograf",
        "Hydrographe",
        "Hygi",
        "Imprimeur lithographe",
        "Infirmi",
        "Infirmier",
        "Infirmier ",
        "Infirmier major pensionn",
        "Informaticien",
        "Ing",
        "Ingeni",
        "Ingenieur",
        "Ingenj",
        "Interne des h",
        "Interne en m",
        "Ishavsskipper",
        "J",
        "Jordbrukskonsulent",
        "Jordemoder",
        "Jordemor",
        "Kapit",
        "Kapitein",
        "Kartarbetare",
        "Kartarbeterska",
        "Kartbitr",
        "Kartfabriksarbeterska",
        "Kartograf",
        "Kartographin",
        "Kartritare",
        "Kartriterska",
        "Kemiker",
        "Kemist",
        "Kemisthustru",
        "Kofferdikonstapelhustru",
        "Kofferdistyrman",
        "Kommissionsavvittringslantm",
        "Kommissionslantm",
        "Konstrukt",
        "Krankengymnastin",
        "Krankenpfleger",
        "Krankenpflegerin",
        "Krankenschwester",
        "Kreisbauaufseher",
        "Kronolots",
        "Kvaksalver",
        "L",
        "Laborant",
        "Laborantine",
        "Laborator",
        "Laboratoriearbetare",
        "Laboratoriearbeterska",
        "Laboratoriebitr",
        "Laboratoriedr",
        "Ladies' nurse",
        "Landtierarzt",
        "Landv",
        "Lantbruksingenj",
        "Lantm",
        "Leg.sjukgymnast",
        "Leichenschauer",
        "Licence en sciences commerciales",
        "Liktornsoperat",
        "Liktornsoperatris",
        "Linjeingenj",
        "Locomotive engineer",
        "Lods",
        "Lots",
        "Lotsdr",
        "Lotsl",
        "M",
        "Machineteekenaar",
        "Machinetekenaar",
        "Maioral de iates",
        "Mariningenj",
        "Marinkartograf",
        "Marktschipper",
        "Maschinenbau-Ingenieur",
        "Maschinenbauer",
        "Maskinexpert",
        "Maskiningenj",
        "Maskinkonstrukt",
        "Maskinritare",
        "Maskintekniker",
        "Mass",
        "Massageelev",
        "Masseur",
        "Masseuse",
        "Master mariner",
        "Matematiker",
        "Math",
        "Matron to the lying in society",
        "Med",
        "Medicine doktor",
        "Medicine filosofie kandidat",
        "Medicine kandidat",
        "Medicine licensiat",
        "Medicine studerande",
        "Mejeriexpert",
        "Mejerikonsulent",
        "Mekaniktecknare",
        "Mestre de hiate",
        "Metge cirugi",
        "Midwife",
        "Mikroskopist",
        "Milchkontrollassistent",
        "Milchkontrolleur",
        "Mining engineer",
        "Monthly nurse",
        "Naturaliste",
        "Navigateur",
        "Navigateur dans l'aviation",
        "Navigationselev",
        "Navigator",
        "Nurse girl",
        "Nutritionniste",
        "Odont",
        "Odont.kand.",
        "Odont.studerande",
        "Odontologista",
        "Officier de marine",
        "Officier de sant",
        "Officier van gezondheid",
        "Oficial da Marinha Mercante",
        "Oficial de marinha",
        "Oficial de navio",
        "Operationssk",
        "Optician",
        "Opticien",
        "Optikarbetare",
        "Optikarbeterska",
        "Optiker",
        "Optikerhustru",
        "Optikerl",
        "Optom",
        "Opzichter tekenaar",
        "Opzigter teekenaar",
        "Orgelingenj",
        "P",
        "PLOIARXOS",
        "Particulier schipper",
        "Particulier schippper",
        "Pauper late midwife",
        "Pfleger",
        "Pfleger(in)",
        "Pflegerin",
        "Pharmacien",
        "Pharmacienne",
        "Physicus",
        "Physioth",
        "Pilot",
        "Pilote",
        "Pilote d'avion",
        "Piloto",
        "Pirot",
        "Pr",
        "Practicante",
        "Privatsjuksk",
        "Privatsk",
        "Prospecteur",
        "Provisor",
        "Pu",
        "Qu",
        "Quimico industrial",
        "Radio-technicien",
        "Ritare",
        "Ritarehustru",
        "Ro",
        "Rote-Kreuz-Schwester",
        "Sage-femme",
        "Sanit",
        "Schiffer",
        "Schifferin",
        "Schiffsf",
        "Schiffskapit",
        "Schipper",
        "Schipperse",
        "Scientifique (sciences commerciales)",
        "Seefahrer",
        "Seelotse",
        "Sergent-pilote",
        "Sick nurse",
        "Sick nurse and knitter of stockings",
        "Sinnessjukv",
        "Sjukgymnast",
        "Sjukgymnasthustru",
        "Sjukhussyssloman",
        "Sjukv",
        "Skeppsbyggare",
        "Skeppsbyggm",
        "Skeppsbyggnadsingenj",
        "Skibsf",
        "Skibskaptein",
        "Sockenbarnmorska",
        "Sota-piloto",
        "Sous-officier de la marine",
        "Stadsingeni",
        "Stadsl",
        "Stadsmeteorolog",
        "Stationsdi",
        "Stationsingenj",
        "Statisticien",
        "Statistiker",
        "Statistikf",
        "Statsagronom",
        "Statsgeodet",
        "Statsmeteorolog",
        "Steuermann",
        "Stuurman",
        "Styrman",
        "Styrmand",
        "Styrmand med dampskib",
        "Styrmand med seilskib",
        "Surgeon",
        "Surveillant",
        "Surveillante ",
        "Surveyor",
        "T",
        "T.f.aktuarie",
        "T.f.stadsl",
        "Tandarts",
        "Tandbitr",
        "Tandl",
        "Tandsk",
        "Tandteknikarbetare",
        "Tandtekniker",
        "Tandteknikerbitr",
        "Tandteknikerhustru",
        "Te",
        "Technicien",
        "Technicien dans l'aviation",
        "Technicien en ",
        "Technicien en alimentation",
        "Technicien en communication",
        "Technicien en industrie laiti",
        "Technicien en laboratoire",
        "Technicien en op",
        "Technicien en pu",
        "Technicien en radiologie",
        "Technicien m",
        "Technicien(ne) m",
        "Technicienne ",
        "Technicienne en tuberculose",
        "Technicienne m",
        "Technicus",
        "Techniker",
        "Tekenaar",
        "Tekniker",
        "Teknikkemist",
        "Teknikl",
        "Teknolog",
        "Telegrafingenj",
        "Teniente de Nav",
        "Textiltechniker",
        "Textiltekniker",
        "Tierarzt",
        "Tinent de Vaixell",
        "Topograf",
        "Tr",
        "Turfschipper",
        "Under nurse",
        "Unterpfleger",
        "Uppfinnare",
        "Uppt",
        "V",
        "Vatteningenj",
        "Vattenl",
        "Vattenverksingenj",
        "Veerman",
        "Veerschipper",
        "Verkstadsingenj",
        "Vermessungstechniker",
        "Veterin",
        "Veterinario",
        "Veterinary practitioner",
        "Veterinary surgeon",
        "Veterniari",
        "Vetinary practitioner",
        "Vetinary surgeon",
        "Vice kommissionslantm",
        "Vrachtjager",
        "Vragtjager",
        "Vroedvrouw",
        "Wehmutter",
        "Werktuigkundig ingenieur",
        "Werktuigkundige",
        "Wijkverpleegster",
        "Wundarzt",
        "Zahnarzt",
        "Zand schipper",
        "Zandschipper",
        "Zeichner",
        "Zeichnerin",
        "a",
        "aanlegger van tuinen",
        "actuaire",
        "adjoint technicien de l'aviation",
        "agent chimiste",
        "agent psychi",
        "agent t",
        "agent technicien",
        "agent technicien d'aviation",
        "agent technique ",
        "agent technique automobile",
        "agent technique de l'",
        "agent technique de la circulation a",
        "agent technique en ",
        "agent vicinal",
        "agent voyer",
        "agent voyer dessinateur",
        "agent voyer en chef",
        "agronome",
        "aide arpenteur",
        "aide chimiste",
        "aide g",
        "aide m",
        "aide manipulateur radiographe",
        "aide pr",
        "aide radiologue",
        "aise",
        "amanuensis aan de rijks hoogere burgerschool",
        "analyst",
        "analyste",
        "analyste programmeur",
        "ancien capitaine de commerce",
        "ancien contrema",
        "ancien pilote",
        "animatrice",
        "animatrice sp",
        "apothecar",
        "apothekersassistent",
        "apothekersbediende",
        "apothekersknecht",
        "artisan opticien",
        "arzt",
        "aspirant d'aviation(",
        "aspirant officier de l'arm",
        "aspirant pilote",
        "assistant de chimie",
        "assistant de laboratoire",
        "assistant technique",
        "assistant v",
        "assistent bij botanie",
        "auxiliaire de pu",
        "auxiliaire pu",
        "aviateur",
        "bakschipper",
        "beurrschipper",
        "beurtschipper",
        "binnenloods",
        "boeyerschipper",
        "bouwkundig opzichter",
        "bouwkundig tekenaar",
        "canicien",
        "canicien de l'a",
        "canicien-aviateur",
        "canique",
        "capitaine au long cours",
        "capitaine de port",
        "chauffagiste",
        "chef de brigade g",
        "chef laborantin",
        "chimiste",
        "chimiste retrait",
        "chirurgie",
        "chirurgien dentiste",
        "chirurgien dentiste retrait",
        "chronom",
        "cialis",
        "cialiste",
        "cin en arm",
        "cktsresande",
        "cnic",
        "cnic T",
        "cnico",
        "cnico Textil",
        "cola",
        "cole d'agriculture",
        "cologue",
        "com",
        "commis g",
        "commis m",
        "communication",
        "communications",
        "conomiste",
        "conseiller agricole",
        "ctrocardiologie m",
        "ctroradiographe m",
        "ctroradiologie",
        "curit",
        "dande barnmorska",
        "dande stadsveterin",
        "de",
        "decin",
        "decin gyn",
        "decin ophtalmologiste",
        "decin sp",
        "decin v",
        "decine",
        "dentiste",
        "dentiste ambulant",
        "dertekniker",
        "dessinateur aux chemins de fer",
        "dessinateur en chaudronnerie",
        "dessinatrice",
        "dg",
        "di",
        "diatre",
        "dical",
        "dicale",
        "dico Cirujano",
        "dico Municipal",
        "dicure",
        "diste",
        "diste retraite",
        "e",
        "e aux malades",
        "e de l'air",
        "electro-techniker",
        "electrotechnicus",
        "employ",
        "entreprise de paysagiste",
        "ergoth",
        "es",
        "frigomann",
        "frigoriste",
        "g",
        "ge",
        "ge de france",
        "geelev",
        "genees-heel- en verloskundige",
        "gepensioneerd loods",
        "ggerska",
        "gingenj",
        "gociant",
        "gsingenj",
        "gteskipper",
        "gyn",
        "heel en vroedmeester",
        "heelmeester",
        "hneraugenausstecher",
        "hongreur",
        "hrer",
        "hydrographe",
        "infirmier ",
        "informaticien",
        "informaticienne",
        "ing",
        "ingenieur",
        "ingenieur bij de gemeentewerken",
        "ingenj",
        "instructeur air france",
        "kaptein",
        "kare",
        "kareassistent",
        "karebitr",
        "kin",
        "kinesith",
        "konom",
        "l",
        "lderman",
        "lectricien",
        "lectricit",
        "lectro m",
        "lectronicien",
        "lectronique",
        "lectrotechnicien",
        "lectrotechnique",
        "leg",
        "lgo",
        "lhavare",
        "ll",
        "loods",
        "loodsschipper",
        "ltsk",
        "m",
        "manipulateur en ",
        "manipulateuren ",
        "marchand apothicaire",
        "masseur",
        "masseur kin",
        "masseuse",
        "maticien",
        "matique",
        "me",
        "melkcontroleur",
        "metra",
        "mico industrial",
        "mographe",
        "monstrateur radiologue",
        "monteur en chauffage",
        "monteur en chauffage central",
        "monteur en chauffage et sanitaire",
        "motorschipper",
        "n",
        "navigateur",
        "ndare",
        "ndler",
        "neur (arpentage)",
        "ng",
        "ngslupsbef",
        "nieur",
        "nieur ",
        "nieur a",
        "nieur adjoint ponts et chauss",
        "nieur agricole",
        "nieur agricole g",
        "nieur agriculteur",
        "nieur agronome",
        "nieur agronome au coll",
        "nieur agronome p",
        "nieur agronome pr",
        "nieur air france",
        "nieur architecte",
        "nieur attache au minist",
        "nieur aux chemins de fer",
        "nieur aux houill",
        "nieur brasserie",
        "nieur chimiste",
        "nieur chimiste ",
        "nieur civil",
        "nieur civil des mines",
        "nieur civil et entrepreneur",
        "nieur dans la construction",
        "nieur de l'institut de physique chimie",
        "nieur de la marine",
        "nieur de s",
        "nieur de travaux",
        "nieur de travaux marine",
        "nieur des eaux et for",
        "nieur des mines",
        "nieur des ponts",
        "nieur des ponts et chauss",
        "nieur des ponts et chaussees",
        "nieur direction travaux",
        "nieur div des travaux",
        "nieur edf",
        "nieur en informatique",
        "nieur en m",
        "nieur en textile",
        "nieur forestier",
        "nieur g",
        "nieur honoraire des travaux publics",
        "nieur hydrographe",
        "nieur informaticien",
        "nieur m",
        "nieur principal",
        "nieur radio",
        "nieur sanitaire",
        "nieur statisticien",
        "nieur textile",
        "nieur travaux publics",
        "nieur-g",
        "nieur-m",
        "niste",
        "nka",
        "nkedoktorinna",
        "nomo",
        "nskild agronomhustru",
        "nskild byggnadsingenj",
        "nskild civilingenj",
        "nskild ingenj",
        "nskild laboratoriearbetarehustru",
        "nskild mass",
        "nskild ritarehustru",
        "nskild tandteknikerhustru",
        "o",
        "o ( navios)",
        "o de navios",
        "od",
        "officier marin",
        "ographe",
        "ologue",
        "om",
        "on chirurgien",
        "ophysique",
        "opticien",
        "opticienne",
        "optom",
        "orologiste",
        "orologue",
        "orthop",
        "ouvrier en parfumerie",
        "ouvrier opticien",
        "ouvrier parfumeur",
        "p",
        "paardendokter",
        "parateur",
        "parateur au coll",
        "parateur en pharmacie",
        "parateur en produit de pharmacie",
        "paration en pharmacie",
        "paratrice en  pharmacie",
        "paratrice en pharmacie",
        "parfumeur",
        "parfumeur distillateur",
        "paysagiste",
        "physicien",
        "pilote",
        "pilote aviateur",
        "pilote civil",
        "pilote d'avion",
        "pilote de ligne",
        "pilote retrait",
        "pini",
        "pital",
        "pital St-Antoine",
        "pital militaire",
        "pitaux",
        "pos",
        "potschipper",
        "pottenschipper",
        "pr",
        "programmeur",
        "programmeur analyste",
        "programmeuse",
        "pu",
        "r",
        "r ved jernbaneanl",
        "r ved ofotjernbanen",
        "radio technicien",
        "radio technicien(us forces)",
        "radiologue",
        "radiotechnicien",
        "rapeute",
        "rapeuthique",
        "rapie",
        "rare",
        "ration th",
        "rdare",
        "rdsarkitekt",
        "rdselev",
        "rdskonsulent",
        "rdslaboratris",
        "re",
        "re classe",
        "re d'industrie",
        "re-hygi",
        "rer",
        "res",
        "rest",
        "rgl",
        "rhuskarl",
        "rhustru",
        "ric",
        "ric T",
        "rico",
        "rico Textil",
        "ricultrice",
        "ricultrice auxiliaire",
        "riculture",
        "rienne",
        "rieur ",
        "rieur des travaux publics",
        "rieur en chimie",
        "rificateur",
        "rificateur du cadastre",
        "rijnschipper",
        "rinaire",
        "rio Municipal",
        "riste",
        "rit Agr",
        "rit Ind",
        "rito Agr",
        "rito Industrial",
        "rl",
        "rling",
        "rnv",
        "ronautique",
        "rselev",
        "rska",
        "rssven",
        "rste aktuarie",
        "rste byr",
        "rste ingenj",
        "rste stadsl",
        "rste stadsveterin",
        "rustend zeeloods",
        "s",
        "scheepsbouwkundig teekenaar",
        "scheepsdocter",
        "scheepsgezagvoerder",
        "scheepskapitein",
        "schipper en koopman",
        "schippers",
        "sensmand",
        "siste",
        "sith",
        "stare",
        "statisticien",
        "sterlots",
        "strial",
        "stuurman ter koopvaardij",
        "t",
        "tallographe",
        "tallographe ",
        "tallurgie",
        "tallurgique",
        "tallurgiste",
        "tandmeester",
        "tar",
        "tare",
        "tareelev",
        "tat",
        "tbef",
        "technicien ",
        "technicien automobile",
        "technicien chimiste",
        "technicien d",
        "technicien de laboratoire",
        "technicien de production",
        "technicien de t",
        "technicien des eaux et for",
        "technicien des t",
        "technicien des travaux forestiers de l'",
        "technicien des travaux publics",
        "technicien du b",
        "technicien du cadastre",
        "technicien en ",
        "technicien en aviation",
        "technicien en b",
        "technicien en chauffage central",
        "technicien en construction",
        "technicien en g",
        "technicien en p",
        "technicien en radio",
        "technicien en radiologie",
        "technicien en soieries",
        "technicien en t",
        "technicien forestier",
        "technicien formateur aux t",
        "technicien frigoriste",
        "technicien g",
        "technicien m",
        "technicien ortf",
        "technicien radio",
        "technicien rtf",
        "technicien sup",
        "technicien travaux publics",
        "teriauskultant",
        "terielev",
        "terska",
        "thermicien",
        "ticienne",
        "timent",
        "tiste",
        "toxicologue",
        "tre",
        "tre arpenteur",
        "tre au cadastre",
        "tre de la mairie",
        "tre de premi",
        "tre du cadastre",
        "tre edf",
        "tre m",
        "tre stagiaire du cadastre",
        "treur",
        "treur v",
        "trique",
        "triste",
        "troles",
        "ts",
        "tsoberfeldwebel",
        "tudiant assistant g",
        "tudiant en biologie",
        "tudiant en chimie",
        "tudiant en math",
        "tudiant en maths",
        "urologue",
        "ve en m",
        "ve en pharmacie",
        "ve ing",
        "veearts",
        "veermansknecht",
        "verrier en laboratoire",
        "vision",
        "vision fran",
        "vroedmeester",
        "xtil",
        "zeeloods" ;
    skos:broader <http://historyofwork.iisg.nl/resource/090> ;
    skos:definition "Conducts research to determine existing level of sales for particular products and services and to assess potential market and future trend."@en ;
    skos:prefLabel "Market Research Analyst"@en .

<http://historyofwork.iisg.nl/resource/11> a skos:Concept ;
    skos:broader <http://historyofwork.iisg.nl/resource/1> ;
    skos:definition "Workers in this minor group plan and direct accounting services, advise on accountancy problems, and plan and conduct financial audits."@en ;
    skos:prefLabel "Accountants"@en .

<http://historyofwork.iisg.nl/resource/12> a skos:Concept ;
    skos:broader <http://historyofwork.iisg.nl/resource/1> ;
    skos:definition "Workers in this minor group plead cases or conduct prosecutions in courts of justice, preside over judicial proceedings and pronounce judgements, give advice on legal matters, draw up legal documents, draft legislation and perform other legal functions."@en ;
    skos:prefLabel "Jurists"@en .

<http://historyofwork.iisg.nl/resource/13> a skos:Concept ;
    skos:broader <http://historyofwork.iisg.nl/resource/1> ;
    skos:definition "Workers in this minor group conduct classes and give private lessons to instruct students at the third, second, first or pre-primary level, educate handicapped persons, undertake research and advise on teaching methods and instructional aids, organise and direct teaching activities in schools, and perform related tasks.In some countries, a stratified system of educational levels is a relatively recent development. In the case of English elementary schools, for example, Teachers might be coded to unit group 1-33, or to 1-30.20. Physical training instructors and sports coaches instructing in educational establishments are classified in unit group 1-80."@en ;
    skos:prefLabel "Teachers"@en .

<http://historyofwork.iisg.nl/resource/14> a skos:Concept ;
    skos:broader <http://historyofwork.iisg.nl/resource/1> ;
    skos:definition "Workers in this minor group minister religion, give spiritual guidance, propagate religious doctrines, perform a variety of other functions associated with the propagation and practice of religions, and endeavour to cure human ailments by the power of faith."@en ;
    skos:prefLabel "Workers In Religion"@en .

<http://historyofwork.iisg.nl/resource/15> a skos:Concept ;
    skos:broader <http://historyofwork.iisg.nl/resource/1> ;
    skos:definition "Workers in this minor group write literary works for publication or dramatic presentation, write critiques of literary, artistic and musical works and of musical, dramatic and other artistic performances, and compose other written material to inform, entertain or influence the public."@en ;
    skos:prefLabel "Authors, Journalists And Related Writers"@en .

<http://historyofwork.iisg.nl/resource/16> a skos:Concept ;
    skos:broader <http://historyofwork.iisg.nl/resource/1> ;
    skos:definition "Workers in this minor group create and execute artistic works by sculpturing, painting, drawing, engraving and etching, apply artistic media to illustrative, decorative and sales promotion purposes, take photographs and direct and operate motion picture and television cameras."@en ;
    skos:prefLabel "Sculptors, Painters, Photographers And Related Creative Artists"@en .

<http://historyofwork.iisg.nl/resource/17> a skos:Concept ;
    skos:broader <http://historyofwork.iisg.nl/resource/1> ;
    skos:definition "Workers in this minor group compose, adapt, conduct and perform musical works and dances; produce, direct and act in theatrical, motion picture and broadcast productions; perform a variety of amusing, mystifying and spectacular acts for the entertainment of circus and other audiences; and provide other forms of public entertainment."@en ;
    skos:prefLabel "Composers And Performing Artists"@en .

<http://historyofwork.iisg.nl/resource/18> a skos:Concept ;
    skos:broader <http://historyofwork.iisg.nl/resource/1> ;
    skos:definition "Workers in this minor group participate for gain in, and regulate the conduct of, public sporting competitions, coach sportsmen in the skills of their sport, instruct persons in the development of their physical fitness and perform various related functions."@en ;
    skos:prefLabel "Athletes, Sportsmen And Related Workers"@en .

<http://historyofwork.iisg.nl/resource/19> a skos:Concept ;
    skos:broader <http://historyofwork.iisg.nl/resource/1> ;
    skos:definition "Workers in this minor group perform professional and technical functions not performed by those classified elsewhere."@en ;
    skos:prefLabel "Professional, Technical And Related Workers Not Elsewhere Classified"@en .

<http://historyofwork.iisg.nl/resource/20> a skos:Concept ;
    skos:broader <http://historyofwork.iisg.nl/resource/2> ;
    skos:definition "Workers in this minor group decide or participate in formulating governmental policy, make, amend or repeal laws and official regulations and direct the administration of government departments to implement government policy and laws, public rules and regulations. They are elected or appointed and work in national, state, provincial or local governments or intergovernmental organisations."@en ;
    skos:prefLabel "Legislative Officials And Government Administrators"@en .

<http://historyofwork.iisg.nl/resource/21> a skos:Concept ;
    skos:broader <http://historyofwork.iisg.nl/resource/2> ;
    skos:definition "Workers in this minor group plan, organise, co-ordinate and direct public and private industrial, commercial, public utility, transport, communications and other undertakings, establishments and organisations (or one or more of their departments). ollow (see, for example, 2-11.10 and 2-12.20), with the exception that: (a) all working proprietors of wholesale and retail businesses are classified in minor group 4-1; (b) all working proprietors of enterprises operating catering and lodging services are classified in minor group 5-1; (c) all farmers are classified in minor group 6-1. Not included in minor group 2-1 are those workers who have the status of working proprietor or who have special titles, including such terms as"@en ;
    skos:prefLabel "Managers"@en .

<http://historyofwork.iisg.nl/resource/22> a skos:Concept ;
    skos:broader <http://historyofwork.iisg.nl/resource/2> ;
    skos:definition "Workers in this minor group organise, supervise and inspect, within industrial and commercial enterprises, public and private organisations, institutions and establishments, the daily tasks and activities of subordinates. They do so subject to the general directives of managers, as listed in minor group"@en ;
    skos:prefLabel "Supervisors, Foremen And Inspectors"@en .

<http://historyofwork.iisg.nl/resource/30> a skos:Concept ;
    skos:broader <http://historyofwork.iisg.nl/resource/3> ;
    skos:definition "Workers in this minor group may perform any (but not all) occupational activities described in minor groups 3-1 to 3-9."@en ;
    skos:prefLabel "Clerical And Related Workers, Specialisation Unknown"@en .

<http://historyofwork.iisg.nl/resource/31> a skos:Concept ;
    skos:broader <http://historyofwork.iisg.nl/resource/3> ;
    skos:definition "Workers in this minor group put into effect government policy decisions and implement laws, rules and regulations under the direction of Government administrators (unit group 2-02). Following the principle of classification according to type of work performed, government employees whose principal functions are to carry out professional, technical and related duties are classified in major group 0/1 and those whose duties consist mainly in supervising clerical work are classified in unit group 2-11. Government employees performing mainly clerical and related work, such as bookkeepers, cashiers, stenographers, typists and telephone or telegraph operators, are classified in minor groups 3-2 to 3-9, and those performing mainly sales, service, production, transport operation or labouring duties are classified, as appropriate, within major groups 4, 5, 6 and 7/8/9."@en ;
    skos:prefLabel "Government Executive Officials"@en .

<http://historyofwork.iisg.nl/resource/32> a skos:Concept ;
    skos:broader <http://historyofwork.iisg.nl/resource/3> ;
    skos:definition "Workers in this minor group record oral or written matter by shorthand and typing and operate card- or tape-punching machines."@en ;
    skos:prefLabel "Stenographers, Typists And Card- And Tape-Punching Machine Operators"@en .

<http://historyofwork.iisg.nl/resource/33> a skos:Concept ;
    skos:broader <http://historyofwork.iisg.nl/resource/3> ;
    skos:definition "Workers in this minor group keep records of business transactions and handle cash on behalf of an organisation and its customers and other persons; calculate costs and wages and perform other specialised bookkeeping and computing clerical duties."@en ;
    skos:prefLabel "Bookkeepers, Cashiers And Related Workers"@en .

<http://historyofwork.iisg.nl/resource/34> a skos:Concept ;
    skos:broader <http://historyofwork.iisg.nl/resource/3> ;
    skos:definition "Workers in this minor group operate bookkeeping, calculating and automatic data-processing machines."@en ;
    skos:prefLabel "Computing Machine Operators"@en .

<http://historyofwork.iisg.nl/resource/36> a skos:Concept ;
    skos:broader <http://historyofwork.iisg.nl/resource/3> ;
    skos:definition "Workers in this minor group take charge of trains, buses and other public transport vehicles during journeys and safeguard passengers."@en ;
    skos:prefLabel "Transport Conductors"@en .

<http://historyofwork.iisg.nl/resource/37> a skos:Concept ;
    skos:broader <http://historyofwork.iisg.nl/resource/3> ;
    skos:definition "Workers in this minor group perform sorting, recording, delivery and other duties in connection with the distribution of mail and the forwarding of messages. They may be employed in public services or private enterprises. Workers primarily engaged in driving vehicles for mail transport are classified in minor group 9-8."@en ;
    skos:prefLabel "Mail Distribution Clerks"@en .

<http://historyofwork.iisg.nl/resource/38> a skos:Concept ;
    skos:broader <http://historyofwork.iisg.nl/resource/3> ;
    skos:definition "Workers in this minor group transmit and receive messages by operating telecommunications equipment on land and sea and in aircraft. Operators of special typewriters such as telex or teleprinter equipment are classified in 3-21.50."@en ;
    skos:prefLabel "Telephone And Telegraph Operators"@en .

<http://historyofwork.iisg.nl/resource/39> a skos:Concept ;
    skos:broader <http://historyofwork.iisg.nl/resource/3> ;
    skos:definition "Workers in this minor group perform various clerical and related duties not elsewhere classified. Included are those who record the receipt, storage, weighing and issuing of finished goods or materials; dispatch, receive, store, issue and weigh materials; prepare orders for materials required for production processes; calculate quantities needed and draw up production schedules; prepare business letters and other correspondence; provide information and services to visitors in agencies; code and compile statistical data; operate office machines for reproducing copies of documents; operate addressing machines; carry out other recording, correspondence and filing tasks."@en ;
    skos:prefLabel "Clerical And Related Workers Not Elsewhere Classified"@en .

<http://historyofwork.iisg.nl/resource/41> a skos:Concept ;
    skos:broader <http://historyofwork.iisg.nl/resource/4> ;
    skos:definition "Workers in this minor group conduct businesses in wholesale and retail trade on their own behalf or in partnership and are engaged in buying and selling goods."@en ;
    skos:prefLabel "Working Proprietors (Wholesale And Retail Trade)"@en .

<http://historyofwork.iisg.nl/resource/42> a skos:Concept ;
    skos:broader <http://historyofwork.iisg.nl/resource/4> ;
    skos:definition "Workers in this minor group buy goods for resale or use on behalf of wholesale, retail, industrial or other establishments or institutions."@en ;
    skos:prefLabel "Buyers"@en .

<http://historyofwork.iisg.nl/resource/43> a skos:Concept ;
    skos:broader <http://historyofwork.iisg.nl/resource/4> ;
    skos:definition "Workers in this minor group carry out specialised technical selling activities requiring knowledge of the technology of the composition, utilisation and maintenance of the goods or equipment sold; sell specialised engineering and assimilated services; give technical information and advice to customers before and after sales; solicit orders and sell goods on a wholesale basis by visiting clients in a defined district; and act as intermediaries for sales on behalf of local or foreign manufacturers to wholesale and retail establishments."@en ;
    skos:prefLabel "Technical Salesmen, Commercial Travellers And Manufacturers Agents"@en .

<http://historyofwork.iisg.nl/resource/44> a skos:Concept ;
    skos:broader <http://historyofwork.iisg.nl/resource/4> ;
    skos:definition "Workers in this minor group sell insurance, real estate, securities, business and advertising services and auction property or commodities, or perform related functions."@en ;
    skos:prefLabel "Insurance, Real Estate, Securities And Business Services Salesmen And Auctioneers"@en .

<http://historyofwork.iisg.nl/resource/45> a skos:Concept ;
    skos:broader <http://historyofwork.iisg.nl/resource/4> ;
    skos:definition "Workers in this minor group sell and demonstrate goods in wholesale or retail establishments or on the street, solicit orders on the street or from door to door and perform related selling tasks."@en ;
    skos:prefLabel "Salesmen, Shop Assistants And Related Workers"@en .

<http://historyofwork.iisg.nl/resource/49> a skos:Concept ;
    skos:broader <http://historyofwork.iisg.nl/resource/4> ;
    skos:definition "Workers in this minor group perform various selling tasks not classified elsewhere."@en ;
    skos:prefLabel "Sales Workers Not Elsewhere Classified"@en .

<http://historyofwork.iisg.nl/resource/51> a skos:Concept ;
    skos:broader <http://historyofwork.iisg.nl/resource/5> ;
    skos:definition "Workers in this minor group conduct catering, lodging and leisure services in establishments ranging from hotels, boarding houses, restaurants and cafes, to recreation rooms, sports halls and fairgrounds, either on their own behalf or in partnership."@en ;
    skos:prefLabel "Working Proprietors (Catering, Lodging And Leisure Services)"@en .

<http://historyofwork.iisg.nl/resource/53> a skos:Concept ;
    skos:broader <http://historyofwork.iisg.nl/resource/5> ;
    skos:definition "Workers in this minor group supervise and perform various kinds of work related to the preparation and cooking of meals and the serving of food and beverages. They may be employed in hotels or other commercial establishments, in institutions or in private households or on board ships or railway trains."@en ;
    skos:prefLabel "Cooks, Waiters, Bartenders And Related Workers"@en .

<http://historyofwork.iisg.nl/resource/54> a skos:Concept ;
    skos:broader <http://historyofwork.iisg.nl/resource/5> ;
    skos:definition "Workers in this minor group provide personal and housekeeping services in private households, hotels and aboard ships, in public conveyances and other establishments."@en ;
    skos:prefLabel "Maids And Related Housekeeping Service Workers Not Elsewhere Classified"@en .

<http://historyofwork.iisg.nl/resource/55> a skos:Concept ;
    skos:broader <http://historyofwork.iisg.nl/resource/5> ;
    skos:definition "Workers in this minor group take care of and clean windows, building interiors, equipment and furniture."@en ;
    skos:prefLabel "Building Caretakers, Charworkers, Cleaners And Related Workers"@en .

<http://historyofwork.iisg.nl/resource/56> a skos:Concept ;
    skos:broader <http://historyofwork.iisg.nl/resource/5> ;
    skos:definition "Workers in this minor group launder, dry clean, press and mend clothing, textile fabrics and similar articles."@en ;
    skos:prefLabel "Launderers, Dry-Cleaners And Pressers"@en .

<http://historyofwork.iisg.nl/resource/57> a skos:Concept ;
    skos:broader <http://historyofwork.iisg.nl/resource/5> ;
    skos:definition "Workers in this minor group cut and dress hair, apply cosmetics and make-up, and perform related tasks to improve the appearance of individuals."@en ;
    skos:prefLabel "Hairdressers, Barbers, Beauticians And Related Workers"@en .

<http://historyofwork.iisg.nl/resource/58> a skos:Concept ;
    skos:broader <http://historyofwork.iisg.nl/resource/5> ;
    skos:definition "Workers in this minor group protect individuals and property against hazards and enforce law and order."@en ;
    skos:prefLabel "Protective Service Workers"@en .

<http://historyofwork.iisg.nl/resource/59> a skos:Concept ;
    skos:broader <http://historyofwork.iisg.nl/resource/5> ;
    skos:definition "Workers in this minor group perform various service tasks not elsewhere classified."@en ;
    skos:prefLabel "Service Workers Not Elsewhere Classified"@en .

<http://historyofwork.iisg.nl/resource/61> a skos:Concept ;
    skos:broader <http://historyofwork.iisg.nl/resource/6> ;
    skos:definition "Workers in this minor group conduct mixed farms to produce a variety of agricultural and animal husbandry products, or specialised farms to produce a particular type of agricultural or animal husbandry product, on their own behalf or in partnership."@en ;
    skos:prefLabel "Farmers"@en .

<http://historyofwork.iisg.nl/resource/62> a skos:Concept ;
    skos:broader <http://historyofwork.iisg.nl/resource/6> ;
    skos:definition "Workers in this minor group perform a variety of tasks in growing field and market garden crops, cultivating trees, shrubs and flowers, breeding and raising livestock and poultry, operating farm machinery and related agricultural and animal husbandry work. Farm supervisors are classified in unit group 2-25 and working proprietors of farms in minor group 6-1."@en ;
    skos:prefLabel "Agricultural And Animal Husbandry Workers"@en .

<http://historyofwork.iisg.nl/resource/63> a skos:Concept ;
    skos:broader <http://historyofwork.iisg.nl/resource/6> ;
    skos:definition "Workers in this minor group supervise and perform tasks in the cultivation, conservation and exploitation of forests."@en ;
    skos:prefLabel "Forestry Workers"@en .

<http://historyofwork.iisg.nl/resource/64> a skos:Concept ;
    skos:broader <http://historyofwork.iisg.nl/resource/6> ;
    skos:definition "Workers in this minor group catch and collect fish, hunt and trap animals, and perform related tasks. Hunting and fishing guides are classified in unit group 5-91 and pelt graders and dressers in unit group 7-62."@en ;
    skos:prefLabel "Fishermen, Hunters And Related Workers"@en .

<http://historyofwork.iisg.nl/resource/71> a skos:Concept ;
    skos:broader <http://historyofwork.iisg.nl/resource/7> ;
    skos:definition "Workers in this minor group extract solid minerals from underground or surface mines and quarries, prepare the extracted minerals for distribution or further processing, and erect and operate drilling plant and perform related tasks in the sinking and operation of wells. Operators of earth-moving equipment in mines and quarries are classified in unit group 9-94; crusher-grinder operators employed in chemical and related processing plants in unit group 7-41; well diggers who works with hand tools in unit group 9-59; and riggers (oil and gas well drilling) in unit group 9-72."@en ;
    skos:prefLabel "Miners, Quarrymen, Well-Drillers And Related Workers"@en .

<http://historyofwork.iisg.nl/resource/72> a skos:Concept ;
    skos:broader <http://historyofwork.iisg.nl/resource/7> ;
    skos:definition "Workers in this minor group operate furnaces to smelt, convert, refine, melt and reheat metals; operate metal-rolling mills; pour metal into moulds and operate metal-casting machines; make sand moulds and cores for casting metal; alter the physical properties of metal objects by heating, cooling and chemical treatment; draw and extrude metals to make wire, pipes, tubes and similar products; operate equipment to plate and coat metal products; and perform related tasks."@en ;
    skos:prefLabel "Metal Processors"@en .

<http://historyofwork.iisg.nl/resource/73> a skos:Concept ;
    skos:broader <http://historyofwork.iisg.nl/resource/7> ;
    skos:definition "Workers in this minor group season and preserve wood; operate machines to saw wood, cut veneer, make plywood and otherwise prepare wood for use; prepare pulp for making paper; and make paper by hand or machine."@en ;
    skos:prefLabel "Wood Preparation Workers And Paper Makers"@en .

<http://historyofwork.iisg.nl/resource/74> a skos:Concept ;
    skos:broader <http://historyofwork.iisg.nl/resource/7> ;
    skos:definition "Workers in this minor group crush, grind, mix, blend, cook, roast, filter, separate, distil, refine and otherwise treat chemicals and other materials used in chemical and related processes."@en ;
    skos:prefLabel "Chemical Processors And Related Workers"@en .

<http://historyofwork.iisg.nl/resource/75> a skos:Concept ;
    skos:broader <http://historyofwork.iisg.nl/resource/7> ;
    skos:definition "Workers in this minor group prepare natural textile fibres for spinning and winding; spin, double, twist and wind thread and yarn; set and maintain weaving and knitting machines and prepare pattern cards; weave materials on hand or machine looms; knit garments, fabrics and other articles by hand or machine; bleach, dye and otherwise treat textile products; and perform related textile fabrics manufacturing tasks."@en ;
    skos:prefLabel "Spinners, Weavers, Knitters, Dyers And Related Workers"@en .

<http://historyofwork.iisg.nl/resource/76> a skos:Concept ;
    skos:broader <http://historyofwork.iisg.nl/resource/7> ;
    skos:definition "Workers in this minor group prepare hides, skins and fur- or wool-bearing pelts for making leather and fur products."@en ;
    skos:prefLabel "Tanners, Fellmongers And Pelt Dressers"@en .

<http://historyofwork.iisg.nl/resource/77> a skos:Concept ;
    skos:broader <http://historyofwork.iisg.nl/resource/7> ;
    skos:definition "Workers in this minor group prepare food products and beverages of all kinds for human and animal consumption."@en ;
    skos:prefLabel "Food And Beverage Processors"@en .

<http://historyofwork.iisg.nl/resource/78> a skos:Concept ;
    skos:broader <http://historyofwork.iisg.nl/resource/7> ;
    skos:definition "Workers in this minor group prepare and treat tobacco leaves and make cigars, cigarettes and other tobacco products."@en ;
    skos:prefLabel "Tobacco Preparers And Tobacco Product Makers"@en .

<http://historyofwork.iisg.nl/resource/79> a skos:Concept ;
    skos:broader <http://historyofwork.iisg.nl/resource/7> ;
    skos:definition "Workers in this minor unit group make, or take part in making, garments, hats, gloves and other articles of textile, fur, leather and similar materials; upholster furniture and the interiors of vehicles and sew textile products for furniture and decoration. Workers who prepare and grade hides, skins and pelts are classified in minor group 7-6. Designers of new garment styles are classified in unit group 1-62."@en ;
    skos:prefLabel "Tailors, Dressmakers, Sewers, Upholsterers And Related Workers"@en .

<http://historyofwork.iisg.nl/resource/80> a skos:Concept ;
    skos:broader <http://historyofwork.iisg.nl/resource/8> ;
    skos:definition "Workers in this minor group make and repair footwear mainly of leather and make saddles, harness and various other kinds of products from leather or similar materials."@en ;
    skos:prefLabel "Shoemakers And Leather Goods Makers"@en .

<http://historyofwork.iisg.nl/resource/81> a skos:Concept ;
    skos:broader <http://historyofwork.iisg.nl/resource/8> ;
    skos:definition "Workers in this minor group make and repair wooden furniture, highly finished wooden fittings and similar objects, set and operate precision woodworking machines to saw, shape, plane, turn and carve wooden products and perform related woodworking tasks not elsewhere classified such as making wooden carts, wheels, patterns, models, casks, and smoking pipes. Wicker furniture maker is classified in unit group 9-42; restorers working on wooden objects of artistic or historical value are classified in unit group 1-61; sawing-machine operators in sawmills and Veneer cutter are classified in unit group 7-32."@en ;
    skos:prefLabel "Cabinetmakers And Related Woodworkers"@en .

<http://historyofwork.iisg.nl/resource/82> a skos:Concept ;
    skos:broader <http://historyofwork.iisg.nl/resource/8> ;
    skos:definition "Workers in this minor group cut and shape stone for building, monumental and ornamental purposes. Sculptor is classified in 1-61.20; Marble setter and Stonemason are classified in 9-51; Stone splitter working at quarry site in 7-12.20; and Lithographic stone engraver in 9-24.15."@en ;
    skos:prefLabel "Stone Cutters And Carvers"@en .

<http://historyofwork.iisg.nl/resource/83> a skos:Concept ;
    skos:broader <http://historyofwork.iisg.nl/resource/8> ;
    skos:definition "Workers in this minor group hammer and forge metal by hand or machine, make tools, dies, patterns and other metal articles, using hand and machine tools, set up metal-cutting machine tools, operate machine tools set up for repetitive work, grind, and sharpen tools and perform various metalworking tasks not performed by workers classified elsewhere. Machinery fitters and machine assemblers are classified in unit groups 8-41; Precision instrument makers in 8-42; Electrical fitters in 8-51; and Electronics fitters in 8-52."@en ;
    skos:prefLabel "Blacksmiths, Toolmakers And Machine-Tool Operators"@en .

<http://historyofwork.iisg.nl/resource/84> a skos:Concept ;
    skos:broader <http://historyofwork.iisg.nl/resource/8> ;
    skos:definition "Workers in this minor group assemble, install, service and repair various types of machinery, metal products, engines and mechanical equipment, and make, service and repair watches, clocks and precision instruments (other than electrical) Electrical fitters and related electrical and electronics workers are classified in minor group 8-5."@en ;
    skos:prefLabel "Machinery Fitters, Machine Assemblers And Precision-Instrument Makers (Except Electrical)"@en .

<http://historyofwork.iisg.nl/resource/85> a skos:Concept ;
    skos:broader <http://historyofwork.iisg.nl/resource/8> ;
    skos:definition "Workers in this minor group fit, assemble, install, maintain and repair electrical and electronic equipment such as electrical motors, generators, instruments, signal transmitters and receivers, in homes, industrial plants and other establishments, and in ships, motor vehicles and aircraft; install and service electrical power transmission cables, telephone and telegraph lines and related equipment."@en ;
    skos:prefLabel "Electrical Fitters And Related Electrical And Electronics Workers"@en .

<http://historyofwork.iisg.nl/resource/86> a skos:Concept ;
    skos:broader <http://historyofwork.iisg.nl/resource/8> ;
    skos:definition "Workers in this minor group operate radio and television broadcasting equipment, install and operate sound-recording and amplifying apparatus and operate cinema projectors."@en ;
    skos:prefLabel "Broadcasting And Sound-Equipment Operators And Cinema Projectionists"@en .

<http://historyofwork.iisg.nl/resource/87> a skos:Concept ;
    skos:broader <http://historyofwork.iisg.nl/resource/8> ;
    skos:definition "Workers in this minor group assemble, fit, install and repair plumbing fixtures, pipes and pipeline systems; form and cut metal parts using flame, electric-arc or other sources of heat; make and repair articles and parts of articles of cold sheet metal; shape, assemble, erect and repair heavy metal members such as girders and plates to form structures or structural frameworks."@en ;
    skos:prefLabel "Plumbers, Welders, Sheet-Metal, And Structural Metal Preparers And Erectors"@en .

<http://historyofwork.iisg.nl/resource/88> a skos:Concept ;
    skos:broader <http://historyofwork.iisg.nl/resource/8> ;
    skos:definition "Workers in this minor group make and repair jewellery and precious metal ware, shape and set gems and engrave designs on jewellery and precious metal ware. Workers who cast precious metal ingots are classified in unit group 7-24, and those who anneal precious metals in unit group 7-26."@en ;
    skos:prefLabel "Jewellers And Precious Metal Workers"@en .

<http://historyofwork.iisg.nl/resource/89> a skos:Concept ;
    skos:broader <http://historyofwork.iisg.nl/resource/8> ;
    skos:definition "Workers in this minor group blow, mould, press and roll shapes from molten glass; cut, grind and finish glass; form ceramics products from class and abrasives; operate furnaces and kilns to make glass; bake ceramics and anneal and temper glass; engrave, etch, paint and decorate glass and ceramics articles; perform other functions in the manufacture of glass and ceramics products."@en ;
    skos:prefLabel "Glass Formers, Potters And Related Workers"@en .

<http://historyofwork.iisg.nl/resource/90> a skos:Concept ;
    skos:broader <http://historyofwork.iisg.nl/resource/9> ;
    skos:definition "Workers in this unit group knead and blend raw rubber and rubber compounds and make articles, such as industrial accessories, footwear, domestic articles, sports and life-saving equipment and pneumatic tires, from natural and synthetic rubber and plastics, by extruding, moulding, laminating and vulcanising. Makers of sewn and stitched garments, gloves, furniture coverings and trimmings of rubber, rubberised or plastic materials are classified in minor group 7-9. Workers treating crude rubber (latex) to coagulate and cure (smoke) it are classified in 7-49.90."@en ;
    skos:prefLabel "Rubber And Plastics Product Makers"@en .

<http://historyofwork.iisg.nl/resource/91> a skos:Concept ;
    skos:broader <http://historyofwork.iisg.nl/resource/9> ;
    skos:definition "Workers in this minor group make boxes, envelopes, bags and other products from paper, paperboard, cardboard, cellophane and similar materials."@en ;
    skos:prefLabel "Paper And Paperboard Products Makers"@en .

<http://historyofwork.iisg.nl/resource/92> a skos:Concept ;
    skos:broader <http://historyofwork.iisg.nl/resource/9> ;
    skos:definition "Workers in this minor group compose type, cast and engrave printing plates and operate printing presses to print text and illustrations on paper, metal, cloth or other material; bind books; develop and print photographic still and motion-picture films; perform other related tasks. Proof Reader is classified in 3-99.40."@en ;
    skos:prefLabel "Printers And Related Workers"@en .

<http://historyofwork.iisg.nl/resource/93> a skos:Concept ;
    skos:broader <http://historyofwork.iisg.nl/resource/9> ;
    skos:definition "Workers in this minor group prepare structural surfaces for painting and apply decorative and protective coatings to buildings, ships, motor vehicles and articles of wood, metal, textile and other materials (except glass and ceramic products). Glass and ceramics painters and decorators are classified in unit group 8-95. Paperhanger is classified in 9-59.25."@en ;
    skos:prefLabel "Painters"@en .

<http://historyofwork.iisg.nl/resource/94> a skos:Concept ;
    skos:broader <http://historyofwork.iisg.nl/resource/9> ;
    skos:definition "Workers in this group are production and related workers who are not classified in any other minor group. Included in this group are craftsmen and specialised workers performing functions requiring application of particular techniques; use of particular tools or machines and abilities and experience in working particular materials in order to make such articles as musical instruments; baskets and brushes; products of cast concrete, asbestos cement, artificial stone and other non-metallic mineral products; objects of cork; linoleum; dolls and stuffed toys; rubber stamps; candles; photographic film and paper; matches; buttons; and various other products. The group also includes those who prepare and stuff skins of animals and birds to give life-like form. Also included are those performing other product-making and processing tasks not elsewhere classified."@en ;
    skos:prefLabel "Production And Related Workers Not Elsewhere Classified"@en .

<http://historyofwork.iisg.nl/resource/95> a skos:Concept ;
    skos:broader <http://historyofwork.iisg.nl/resource/9> ;
    skos:definition "Workers in this minor group erect and repair buildings and other structures. They lay bricks, stones and tiles; erect reinforced concrete frameworks; cover roof frameworks with roofing tiles and other materials; make, erect, fit and repair wooden structural frameworks, flooring, fixtures, panelling, boats, plain furniture, and other objects of wood; apply lath and plasters in buildings; apply insulating materials to buildings, boilers, pipes, refrigeration and air-conditioning equipment; fit and set glass in buildings and vehicles; perform other tasks related to building and construction. Plumber and pipe fitters, Welders and flame-cutters, Sheet-metal workers and Structural metal preparers and erectors are classified in minor group 8-7, Crane and hoist operators and Earth-moving and related machinery operators in minor group 9-7, and Building painter in 9-31.20."@en ;
    skos:prefLabel "Bricklayers, Carpenters And Other Construction Workers"@en .

<http://historyofwork.iisg.nl/resource/96> a skos:Concept ;
    skos:broader <http://historyofwork.iisg.nl/resource/9> ;
    skos:definition "Workers in this minor group operate equipment to produce electric power and control its distribution; operate and tend stationary engines and related equipment such as steam boilers, air and gas compressors, pumps, refrigeration plant, heating and ventilation systems and water treatment, waste disposal and similar types of equipment."@en ;
    skos:prefLabel "Stationary Engine And Related Equipment Operators"@en .

<http://historyofwork.iisg.nl/resource/97> a skos:Concept ;
    skos:broader <http://historyofwork.iisg.nl/resource/9> ;
    skos:definition "Workers in this minor group perform freight handling tasks, such as loading and unloading ship and aircraft cargoes and other freight, including petroleum, wrapping objects, packing liquids, material and objects in containers, affixing labels and making marks on containers and operating baling presses; rig cables, wires and ropes for lifting, hauling and other purposes, and splice cables; operate cranes and other hoisting equipment; operate machines to excavate, grade, level and compact earth, mix concrete and lay road surfaces of asphalt and concrete; operate specialised vehicles (not used for road transport) to lift, move, dump and stack materials in warehouses, on mining and construction sites and in timber yards and other establishments; and perform related tasks such as operating conveyors and aerial ropeways."@en ;
    skos:prefLabel "Material Handling And Related Equipment Operators, Dockers And Freight Handlers"@en .

<http://historyofwork.iisg.nl/resource/98> a skos:Concept ;
    skos:broader <http://historyofwork.iisg.nl/resource/9> ;
    skos:definition "Workers in this minor group drive vehicles and perform assimilated tasks related to the transport of passengers and freight by water-borne craft, land transport and pack animals. They carry out deck and engine-room duties aboard ship (under the direction of ships' officers, classified in 0-42 and 0-43) and aboard other water-borne craft, drive locomotives, manoeuvre railway coaches and wagons, operate railway signals and lighthouses, drive motor vehicles and motor-cycles, drive pack animals and vehicles drawn by animas, operate locks in canals and ports, dry-dock vessels, drive pedal vehicles and pull rickshaws and handcarts. Aircraft and ships' officers (including ships' deck officers and engineer officers) are classified in minor group 0-4; Ship's carpenter in 9-54.55. Ship's engine-room mechanics are classified in 8-49.90. Transport conductors are classified in minor group 3-6."@en ;
    skos:prefLabel "Transport Equipment Operators"@en .

<http://historyofwork.iisg.nl/resource/99> a skos:Concept ;
    skos:broader <http://historyofwork.iisg.nl/resource/9> ;
    skos:definition "Workers in this minor group perform manual tasks having a simple and routine nature and requiring mainly physical effort, which are not performed by workers classified elsewhere. Workers performing simple manual tasks in farming and mining are classified in minor group 6-2 and 7-1 respectively; caretakers and cleaners of residences and commercial and other establishments in minor group 5-5; hotel baggage porters in 5-99.90; Dockers and freight handlers in unit group 9-71."@en ;
    skos:prefLabel "Workers Not Elsewhere Classified"@en .

<http://historyofwork.iisg.nl/resource/020> a skos:Concept ;
    skos:broader <http://historyofwork.iisg.nl/resource/02> ;
    skos:definition "Workers in this unit group may perform any (but not all) of the occupational activities listed in unit groups 0-22 to 0-29."@en ;
    skos:prefLabel "Engineers, Specialisation Unknown"@en .

<http://historyofwork.iisg.nl/resource/032> a skos:Concept ;
    skos:broader <http://historyofwork.iisg.nl/resource/03> ;
    skos:definition "Workers in this unit group may perform any (but not all) of the occupational activities described in unit groups 0-14 and 0-33 to 0-39."@en ;
    skos:prefLabel "Technicians, Specialisation Unknown"@en .

<http://historyofwork.iisg.nl/resource/062> a skos:Concept ;
    skos:broader <http://historyofwork.iisg.nl/resource/06> ;
    skos:definition "Workers in this unit group perform, within a public health service or institution, limited diagnostic, preventive and curative medical tasks, mainly in connection with the common diseases of the region. They may work independently or under the general direction of a fully qualified physician. Their theoretical and practical training in medicine is less than that of fully qualified physicians (classified in 0-61). In some countries the functions of medical assistants are carried out solely by physicians."@en ;
    skos:prefLabel "Medical Assistants"@en .

<http://historyofwork.iisg.nl/resource/066> a skos:Concept ;
    skos:broader <http://historyofwork.iisg.nl/resource/06> ;
    skos:definition "Workers in this unit group perform limited diagnostic, preventive and curative veterinary tasks to assist veterinarians, or independently. Their theoretical and practical training in veterinary medicine is less than that of Veterinarians (0-65)."@en ;
    skos:prefLabel "Veterinary Assistants"@en .

<http://historyofwork.iisg.nl/resource/067> a skos:Concept ;
    skos:broader <http://historyofwork.iisg.nl/resource/06> ;
    skos:definition "Workers in this unit group make and dispense medicaments and related preparations according to doctors' prescriptions or established formulae and perform related tasks."@en ;
    skos:prefLabel "Pharmacists"@en .

<http://historyofwork.iisg.nl/resource/068> a skos:Concept ;
    skos:broader <http://historyofwork.iisg.nl/resource/06> ;
    skos:definition "Workers in this unit group assist pharmacists in the making and dispensing of medicaments in pharmacies, hospitals and dispensaries. Their theoretical and practical training in pharmacy is less than that of fully qualified Pharmacist (0-67.10)."@en ;
    skos:prefLabel "Pharmaceutical Assistants"@en .

<http://historyofwork.iisg.nl/resource/072> a skos:Concept ;
    skos:broader <http://historyofwork.iisg.nl/resource/07> ;
    skos:definition "Workers in this unit group provide simple nursing services for patients, generally under the supervision of a physician or professional nurse. They do not have the full training and theoretical knowledge of Professional nurses (0-71)."@en ;
    skos:prefLabel "Nursing Personnel Not Elsewhere Classified"@en .

<http://historyofwork.iisg.nl/resource/073> a skos:Concept ;
    skos:broader <http://historyofwork.iisg.nl/resource/07> ;
    skos:definition "Workers in this unit group provide professional midwifery services in hospitals, clinics and elsewhere, including giving advice and assistance to women during childbirth, providing prenatal and postnatal nursing care of mother and infant, and participating in some aspects of health education."@en ;
    skos:prefLabel "Professional Midwives"@en .

<http://historyofwork.iisg.nl/resource/074> a skos:Concept ;
    skos:broader <http://historyofwork.iisg.nl/resource/07> ;
    skos:definition "Workers in this unit group provide practical midwifery services as a rule in private homes, when there is no physician in attendance, in apparently normal obstetric cases. Their general functions are similar to those of Professional midwives (0-73) but they do not have the full training and theoretical knowledge of the latter."@en ;
    skos:prefLabel "Midwifery Personnel Not Elsewhere Classified"@en .

<http://historyofwork.iisg.nl/resource/077> a skos:Concept ;
    skos:broader <http://historyofwork.iisg.nl/resource/07> ;
    skos:definition "Workers in this unit group operate X-ray equipment to make radiographs for medical diagnostic purposes or to give therapeutic treatment. Industrial radiographer is classified in 0-39.90."@en ;
    skos:prefLabel "Medical X-Ray Technicians"@en .

<http://historyofwork.iisg.nl/resource/083> a skos:Concept ;
    skos:broader <http://historyofwork.iisg.nl/resource/08> ;
    skos:definition "Workers in this unit group analyse data-processing needs and problems of commercial, industrial and other business enterprises, and of research, administrative and other organisations, advise on the feasibility and cost of using automatic data-processing (A.D.P.), and devise and introduce appropriate A.D.P. systems and procedures."@en ;
    skos:prefLabel "Systems Analysts"@en .

<http://historyofwork.iisg.nl/resource/09> a skos:Concept ;
    skos:broader <http://historyofwork.iisg.nl/resource/0> ;
    skos:definition "Workers in this minor group conduct research and apply the principles and theories of economics to formulate solutions to economic problems such as problems of economic development, resources allocation, production, productivity, finance, trade, wages and incomes policies, prices, consumption or marketing."@en ;
    skos:prefLabel "Economists"@en .

<http://historyofwork.iisg.nl/resource/075> a skos:Concept ;
    skos:broader <http://historyofwork.iisg.nl/resource/07> ;
    skos:definition "Workers in this unit group prescribe and fit spectacles and perform related tasks. Their functions include: examining eyes and prescribing spectacles or treatment not involving the use of medicines, surgery or drugs, to conserve or improve vision; assisting customers in choice of spectacle frames, fitting prescribed lenses into frames, and fitting frames or contact lenses to customers."@en ;
    skos:prefLabel "Optometrists and Opticians"@en .

<http://historyofwork.iisg.nl/resource/084> a skos:Concept ;
    skos:broader <http://historyofwork.iisg.nl/resource/08> ;
    skos:definition "Workers in this unit group prepare programmes to control the automatic processing of data by computer and perform other technical tasks contributory to the work of, and normally under the direction and supervision of, statisticians, mathematicians and actuaries."@en ;
    skos:prefLabel "Statistical and Mathematical Technicians"@en .

<http://historyofwork.iisg.nl/resource/021> a skos:Concept ;
    skos:broader <http://historyofwork.iisg.nl/resource/02> ;
    skos:definition "Workers in this unit group design and supervise the construction of buildings; plan layout and co-ordinate development of urban areas; and plan, design and supervise aesthetic landscaping for parks, road development and other projects."@en ;
    skos:prefLabel "Architects and Town Planners"@en .

<http://historyofwork.iisg.nl/resource/025> a skos:Concept ;
    skos:broader <http://historyofwork.iisg.nl/resource/02> ;
    skos:definition "Workers in this unit group carry out research, develop and advise on processes for producing on a commercial scale the chemical or physical transformation of substances, as in manufacture of chemicals, petroleum derivatives, metals, food products and synthetic materials, and design appropriate manufacturing plant and plan and supervise its construction, operation, maintenance and repair."@en ;
    skos:prefLabel "Chemical Engineers"@en .

<http://historyofwork.iisg.nl/resource/026> a skos:Concept ;
    skos:broader <http://historyofwork.iisg.nl/resource/02> ;
    skos:definition "Workers in this unit group advise on metallurgical problems and develop and control processes for the extraction of metals from their ores, study the properties and engineering characteristics of metals and develop new alloys, and develop and supervise metal manufacturing processes for making finished metal products."@en ;
    skos:prefLabel "Metallurgists"@en .

<http://historyofwork.iisg.nl/resource/036> a skos:Concept ;
    skos:broader <http://historyofwork.iisg.nl/resource/03> ;
    skos:definition "Workers in this unit group perform technical tasks, normally under the direction and supervision of chemical engineers, contributory to development of industrial chemical processes and design, construction, operation, maintenance and repair of chemical plant. Their functions include: assisting in research to develop new or improved processes and manufacturing plant for the chemical or physical transformation of substances on a commercial scale; preparing detailed estimates of quantities and costs of materials and labour required for manufacture and installation of plant; assisting with technical supervision of construction, installation, operation, maintenance and repair of plant; applying knowledge of chemical engineering theory and practices to recognise and solve problems arising in the course of their work."@en ;
    skos:prefLabel "Chemical Engineering Technicians"@en .

<http://historyofwork.iisg.nl/resource/038> a skos:Concept ;
    skos:broader <http://historyofwork.iisg.nl/resource/03> ;
    skos:definition "Workers in this unit group perform technical tasks, normally under the direction and supervision of mining engineers, contributory to the extraction from the earth and preparation for distribution or processing of minerals such as coal, iron, copper, gold, platinum, silver, petroleum, gas, stone, clay, salt and diamonds. Their functions include: assisting in geological and topographical surveys; assisting in planning and supervising construction of mine shafts, tunnels and surface developments; assisting in technical supervision of mining and quarrying operations, preparation of minerals for distribution, well-drilling operations and initial treatment of crude oil and natural gas; assisting in research to develop improved methods of extraction; applying knowledge of theory and practices of mining and well-drilling to recognise and solve problems arising in the course of their work."@en ;
    skos:prefLabel "Mining Technicians"@en .

<http://historyofwork.iisg.nl/resource/039> a skos:Concept ;
    skos:broader <http://historyofwork.iisg.nl/resource/03> ;
    skos:definition "Workers in this unit group perform technical functions in engineering, normally under the direction and supervision of engineers, and are not elsewhere classified. Their functions include: assisting industrial engineers in connection with production engineering matters, time and motion studies, or safety measures and procedures; assisting manufacturing technologists specialising in ceramics and glass, food and drink, textiles, paper, leather or wood products, in connection with the development of plant and processes and technical supervision of processing operations; assisting agricultural engineers; assisting traffic planners; performing other technical tasks in engineering."@en ;
    skos:prefLabel "Engineering Technicians Not Elsewhere Classified"@en .

<http://historyofwork.iisg.nl/resource/04> a skos:Concept ;
    skos:broader <http://historyofwork.iisg.nl/resource/0> ;
    skos:definition "Workers in this minor group pilot and navigate aircraft, give instruction in flying aircraft, inspect, adjust and regulate during flight the mechanical equipment of aircraft, command and navigate ships and hovercraft, direct and supervise engine-room activities on board ship, and direct marine services and supplies or mechanical overhauls, replacements and repairs for vessels of a shipping line in port."@en ;
    skos:prefLabel "Aircraft And Ships' Officers"@en .

<http://historyofwork.iisg.nl/resource/043> a skos:Concept ;
    skos:broader <http://historyofwork.iisg.nl/resource/04> ;
    skos:definition "Workers in this unit group plan, co-ordinate, direct and participate in the operation, maintenance and repair of mechanical and related equipment on board ship, or direct from shore station mechanical overhauls, replacements and repairs in port for vessels of a shipping line. Their functions include: taking complete charge of ship's engine-room department, standing watch in engine or boiler room and supervising engine-room department personnel engaged in operation, maintenance and repair of shipboard machinery and equipment; directing from shore station the maintenance and replacement programme and repair work in port for machinery and equipment of vessels of a shipping line."@en ;
    skos:prefLabel "Ships' Engineers"@en .

<http://historyofwork.iisg.nl/resource/063> a skos:Concept ;
    skos:broader <http://historyofwork.iisg.nl/resource/06> ;
    skos:definition "Workers in this unit group apply medical knowledge to the prevention, diagnosis and treatment of human dental or oral disorders. Their functions include: performing diagnostic, preventive and curative services for dental or oral diseases and disorders; giving surgical, medical and other forms of treatment for particular types of dental and oral diseases and disorders; planning and directing public action to improve oral health and to control and improve standards of dental care and treatment of oral disorders."@en ;
    skos:prefLabel "Dentists"@en .

<http://historyofwork.iisg.nl/resource/064> a skos:Concept ;
    skos:broader <http://historyofwork.iisg.nl/resource/06> ;
    skos:definition "Workers in this unit group perform limited diagnostic, curative and preventive dental tasks within a public dental health service (e.g. for schoolchildren), or otherwise. Their theoretical and practical training in dentistry is less than that of Dentists (0-63).Dental prosthesis maker and repairer is classified in 8-42.50. Dental chair-side assistants (workers who help the dentist in his consulting room at the chairside by preparing and taking care of instruments and other dental equipment, preparing materials and looking after the welfare of patients) are classified in unit group 5-99."@en ;
    skos:prefLabel "Dental Assistants"@en .

<http://historyofwork.iisg.nl/resource/065> a skos:Concept ;
    skos:broader <http://historyofwork.iisg.nl/resource/06> ;
    skos:definition "Workers in this unit group diagnose and give or prescribe medical or surgical treatment of diseases, injuries or other medical conditions of animals, and assist in epidemiological, radiological and other surveillance of animal health. Their functions include: diagnosing diseases or injuries of animals; administering surgical or medical treatment; testing dairy and other herds and inoculating animals against disease; advising on care and breeding of animals; performing other functions requiring a scientific knowledge of veterinary medicine such as examining animals for soundness, veterinarian legal work, food hygiene, control of communicable animal diseases and comparative medicine. Veterinary pathologist is classified in 0-52.65."@en ;
    skos:prefLabel "Veterinarians"@en .

<http://historyofwork.iisg.nl/resource/069> a skos:Concept ;
    skos:broader <http://historyofwork.iisg.nl/resource/06> ;
    skos:definition "Workers in this unit group plan and supervise the preparation of diets for individuals or groups, supervise and evaluate nutrition elements of health programmes and assist in appraising the various factors related to nutrition and food problems in the community. Their functions include: planning and supervising the preparation of therapeutic or other diets for individuals or for groups in hospitals, institutions and other establishments and for workers in particular sectors; participating in programmes of nutrition education and in nutrition rehabilitation activities; planning and co-ordinating nutrition programmes and advising on nutrition aspects of community food problems and health programmes."@en ;
    skos:prefLabel "Dietitians and Public Health Nutritionists"@en .

<http://historyofwork.iisg.nl/resource/076> a skos:Concept ;
    skos:broader <http://historyofwork.iisg.nl/resource/07> ;
    skos:definition "Workers in this unit group provide special medical therapeutic services. Their functions include: treating sprains, healing fractures, paralysis and circulatory or nervous disorders by physical means, usually as prescribed by a physician; participating in planned medically oriented vocational, educational or recreational activities designed to rehabilitate physically or mentally disabled persons; massaging clients or patients to improve circulation, soothe or stimulate nerves, facilitate elimination of waste matter, stretch contracted tendons and produce other therapeutic effects."@en ;
    skos:prefLabel "Physiotherapists and Occupational Therapists"@en .

<http://historyofwork.iisg.nl/resource/081> a skos:Concept ;
    skos:broader <http://historyofwork.iisg.nl/resource/08> ;
    skos:definition "Workers in this unit group conduct research into the mathematical basis of the science of statistics; develop new and improved statistical methodology; advise on practical applications of statistical methods; plan and conduct statistical surveys; apply statistical techniques to evaluate, organise, analyse and interpret numerical data obtained from special surveys or other sources."@en ;
    skos:prefLabel "Statistician"@en .

<http://historyofwork.iisg.nl/resource/090> a skos:Concept ;
    skos:broader <http://historyofwork.iisg.nl/resource/09> ;
    skos:definition "Workers in this unit group conduct research and apply the principles and theories of economics to formulate solutions to economic problems arising from production, distribution and exchange of goods and services and referring to such matters as composition of production, markets, trade trends, pricing policies, credit structures, consumption, investment of capital, wages and productivity, and advise on economic questions in a specialised field such as finance, taxation, international trade, labour, agriculture or industrial production and investigate present and potential market for particular goods and services."@en ;
    skos:prefLabel "Economists"@en .

<http://historyofwork.iisg.nl/resource/01> a skos:Concept ;
    skos:broader <http://historyofwork.iisg.nl/resource/0> ;
    skos:definition "Workers in this minor group conduct pure and applied research and develop practical applications of scientific knowledge, or perform related auxiliary technical tasks, in the field of the physical sciences. They normally specialise in a particular branch of physical science, such as organic, inorganic, physical or analytical chemistry, mechanics, heat, light, sound, electricity and magnetism, electronics, nuclear physics, geophysics, geology, meteorology and astronomy, and they may specialise in developing practical applications in medical, industrial, military or other particular fields."@en ;
    skos:prefLabel "Physical Scientists And Related Technicians"@en .

<http://historyofwork.iisg.nl/resource/014> a skos:Concept ;
    skos:broader <http://historyofwork.iisg.nl/resource/01> ;
    skos:definition "Workers in this unit group perform auxiliary technical tasks, normally under the direction and supervision of physical scientists, in connection with research in the physical sciences and the development of industrial, medical, military and other practical applications. Their functions include: preparing materials and equipment for experiments, tests and analyses; assisting with or - under supervision - performing experiments, tests and analyses in such fields as physics, chemistry, geology, geophysics, meteorology and astronomy; applying knowledge of scientific principles to suggest solutions to problems encountered; taking records, making calculations, preparing charts and graphs and writing reports."@en ;
    skos:prefLabel "Physical Science Technicians"@en .

<http://historyofwork.iisg.nl/resource/028> a skos:Concept ;
    skos:broader <http://historyofwork.iisg.nl/resource/02> ;
    skos:definition "Workers in this unit group study, advise on and implement methods to promote the efficient, safe and economic utilisation of personnel, materials and equipment. Their functions include: studying and advising on the organisation and layout of, and methods employed in, production processes and commercial and administrative procedures; planning and conducting time and motion studies; developing work measurement methodology; advising on and initiating measures to prevent industrial accidents and diseases."@en ;
    skos:prefLabel "Industrial Engineers"@en .

<http://historyofwork.iisg.nl/resource/037> a skos:Concept ;
    skos:broader <http://historyofwork.iisg.nl/resource/03> ;
    skos:definition "Workers in this unit group perform technical tasks, normally under direction and supervision of metallurgists, contributory to development and control of processes for extraction of metals from their ores and metal refining, research into properties of metals, development of new alloys, and technical supervision of metal and alloy manufacture and processing."@en ;
    skos:prefLabel "Metallurgical Technicians"@en .

<http://historyofwork.iisg.nl/resource/05> a skos:Concept ;
    skos:broader <http://historyofwork.iisg.nl/resource/0> ;
    skos:definition "Workers in this minor group conduct pure and applied research and develop practical applications of scientific knowledge, or perform related auxiliary technical tasks, in the field of the life sciences. They normally specialise in a particular branch of life sciences, such as biology, botany, zoology, anatomy, biochemistry, physiology, pharmacology, pathology, animal genetics and ecology, agronomy, silviculture, horticulture or pisciculture. They may specialise in developing practical applications in medical, industrial, agricultural and other particular fields."@en ;
    skos:prefLabel "Life Scientists And Related Technicians"@en .

<http://historyofwork.iisg.nl/resource/051> a skos:Concept ;
    skos:broader <http://historyofwork.iisg.nl/resource/05> ;
    skos:definition "Workers in this unit group conduct pure research into all forms of life to increase scientific knowledge and applied research to develop practical applications in fields such as medicine, agriculture and forestry. Their functions include: planning and conducting field and laboratory studies of the origin, development, functions, structure, distribution, environment, interrelationships and other aspects of life-forms; co-ordinating, analysing and evaluating data obtained and preparing reports of findings and conclusions for use in such fields as medicine, agriculture, forestry and pharmaceuticals manufacture."@en ;
    skos:prefLabel "Biologists, Zoologists and Related Scientists"@en .

<http://historyofwork.iisg.nl/resource/054> a skos:Concept ;
    skos:broader <http://historyofwork.iisg.nl/resource/05> ;
    skos:definition "Workers in this unit group perform technical tasks, normally under the direction and supervision of life scientists, contributory to research to increase scientific knowledge in the life sciences and to develop industrial, agricultural, medical and other practical applications. Their functions include: preparing biological, botanical, medical and similar specimens and growing cultures of micro-organisms for tests, analyses and experiments; using laboratory instruments and other equipment to carry out, under supervision or according to instructions, tests, analyses and experiments and recording observations, results and other relevant information; performing other technical tasks to assist life scientists in research and in development of practical applications of life sciences, including sciences of biology, botany, zoology, anatomy, biochemistry, physiology, bacteriology, pathology, pharmacology, agronomy, horticulture and silviculture."@en ;
    skos:prefLabel "Life Sciences Technicians"@en .

<http://historyofwork.iisg.nl/resource/08> a skos:Concept ;
    skos:broader <http://historyofwork.iisg.nl/resource/0> ;
    skos:definition "Workers in this minor group conduct research in the science of statistics to develop new and improved statistical methodology, advise on practical applications of statistical methods, plan and conduct statistical surveys and evaluate, organise and interpret statistical data; conduct research in fundamental mathematics, develop and improve mathematical techniques, advise on application of mathematical techniques for solution of problems in specific fields; apply knowledge of mathematics, statistics and financial affairs to the design and operation of insurance and pensions schemes; analyse data-processing needs and problems of business enterprises and other organisations, advise on and introduce mechanical, semi-automatic and automatic data-processing systems; prepare programmes to control automatic processing of data by computer; and perform technical tasks contributory to the work of statisticians, mathematicians and actuaries."@en ;
    skos:prefLabel "Statisticians, Mathematicians, Systems Analysts And Related Technicians"@en .

<http://historyofwork.iisg.nl/resource/082> a skos:Concept ;
    skos:broader <http://historyofwork.iisg.nl/resource/08> ;
    skos:definition "Workers in this unit group conduct research in fundamental mathematics to advance mathematical knowledge and develop and improve mathematical techniques; advise on practical applications of mathematical principles and techniques to solution of specific problems in scientific research, engineering, logistics, computer applications and other areas; conduct logical analyses of management problems and formulate mathematical models for programming and solution by computer; apply knowledge of mathematics, statistics and financial affairs to design and operation of pensions schemes and life, health, social and casualty insurance systems."@en ;
    skos:prefLabel "Mathematicians and Actuaries"@en .

<http://historyofwork.iisg.nl/resource/013> a skos:Concept ;
    skos:broader <http://historyofwork.iisg.nl/resource/01> ;
    skos:definition "Workers in this unit group conduct research and develop practical applications in areas of the physical sciences not covered by those classified elsewhere. Their functions include: conducting research into the physical nature of the earth, the nature and history of the earth's crust and the physical nature and properties of the atmosphere and the forces affecting it, and developing practical applications in such fields as radio communications, water conservation, mineral exploitation, civil engineering and weather forecasting; observing and interpreting celestial phenomena and developing practical applications in such fields as navigation and space exploration; examining, analysing and classifying minerals and advising on the likely commercial yield of mineral deposits containing gems and precious stones."@en ;
    skos:prefLabel "Physical Scientists Not Elsewhere Classified"@en .

<http://historyofwork.iisg.nl/resource/027> a skos:Concept ;
    skos:broader <http://historyofwork.iisg.nl/resource/02> ;
    skos:definition "Workers in this unit group carry out research on mining engineering problems, supervise prospecting for minerals such as coal, iron, copper, gold, platinum, silver, petroleum, gas, stone, clay, salt or gems, and plan, organise, supervise and advise on extraction of minerals from the earth and their preparation for distribution or processing. Workers who specialise in geological and geophysical surveys to locate mineral deposits are classified in unit group 0-13."@en ;
    skos:prefLabel "Mining Engineers"@en .

<http://historyofwork.iisg.nl/resource/029> a skos:Concept ;
    skos:broader <http://historyofwork.iisg.nl/resource/02> ;
    skos:definition "Workers in this unit group perform engineering functions not performed by those classified elsewhere. Their functions include: studying, designing, developing, controlling and advising on processes and plant for the manufacture of bricks, pottery, glassware, foods or beverages; studying, advising on and supervising the application of engineering technology to agricultural problems; studying, planning and advising on the routing and control of road traffic to promote safety and minimise congestion."@en ;
    skos:prefLabel "Engineers Not Elsewhere Classified"@en .

<http://historyofwork.iisg.nl/resource/033> a skos:Concept ;
    skos:broader <http://historyofwork.iisg.nl/resource/03> ;
    skos:definition "Workers in this unit group perform technical tasks, normally under the direction and supervision of civil engineers, building architects or surveyors, contributory to planning and execution of building and civil engineering projects, including new construction, repair and maintenance. Their functions include: estimating quantities and costs of building materials and labour required for execution of construction projects and preparing bills of quantities; performing technical tasks contributory to execution of surveys and preparation of survey reports; representing building architects on construction sites to ensure compliance with design specifications and maintenance of desired standards of materials and workmanship; applying knowledge of building and civil engineering theory and practices to recognise and solve problems arising in the course of their work. Civil engineering draughtsman is classified in 0-31.40 and Architectural draughtsman in 0-31.50."@en ;
    skos:prefLabel "Civil Engineering Technicians"@en .

<http://historyofwork.iisg.nl/resource/034> a skos:Concept ;
    skos:broader <http://historyofwork.iisg.nl/resource/03> ;
    skos:definition "Workers in this unit group perform technical tasks, normally under the direction and supervision of electrical or electronics engineers, contributory to the design, development, construction, installation, maintenance and repair of electrical and electronic systems and equipment. Their functions include: assisting in research and development work concerning electrical and electronic systems and equipment; preparing detailed estimates of quantities and costs of materials and labour required for manufacture and installation; assisting with technical supervision of manufacture, installation and utilisation, maintenance and repair of electrical and electronic systems and equipment; applying knowledge of electrical and electronics engineering theory and practices to recognise and solve problems arising in course of their work. Electrical fitters, electronics fitters, radio and television repairmen and related workers are classified in minor group 8-5."@en ;
    skos:prefLabel "Electrical and Electronics Engineering Technicians"@en .

<http://historyofwork.iisg.nl/resource/071> a skos:Concept ;
    skos:broader <http://historyofwork.iisg.nl/resource/07> ;
    skos:definition "Workers in this unit group provide professional nursing services. Their functions include: providing professional nursing care and advice in hospitals, clinics or other establishments providing medical care and treatment; providing professional nursing care and advice in private homes, schools, maternal and child health centres and nurseries; providing nursing services and health information for employees in workplaces; performing related tasks."@en ;
    skos:prefLabel "Professional Nurses"@en .

<http://historyofwork.iisg.nl/resource/079> a skos:Concept ;
    skos:broader <http://historyofwork.iisg.nl/resource/07> ;
    skos:definition "Workers in this unit group provide professional medical, dental, veterinary and related services not performed by those classified elsewhere. Their functions include: diagnosing and treating, mainly by manipulative methods, disorders of bones, muscles, blood vessels and other tissues of the human body; relieving illness believed due to pressure upon nervous system at the spine by adjusting joints of the spine; promoting, and supervising implementation of, measures to restore or improve sanitary environmental conditions; writing specifications for and fitting artificial limbs, braces and other appliances for body deformities and disorders following prescription of physician; performing related tasks."@en ;
    skos:prefLabel "Medical, Dental, Veterinary and Related Workers Not Elsewhere Classified"@en .

<http://historyofwork.iisg.nl/resource/011> a skos:Concept ;
    skos:broader <http://historyofwork.iisg.nl/resource/01> ;
    skos:definition "Workers in this unit group conduct research in such fields as organic, inorganic, physical and analytical chemistry. Their functions include: conducting pure research to increase scientific knowledge in the field of chemistry; conducting applied research and development work to test, develop and improve materials, products and industrial processes; performing chemical tests and analyses for process and quality control; developing analytical methodology and techniques. Metallurgists are classified in unit group 0-26, Biochemists and Pharmacologists in 0-52 and Pharmacists in 0-67."@en ;
    skos:prefLabel "Chemists"@en .

<http://historyofwork.iisg.nl/resource/023> a skos:Concept ;
    skos:broader <http://historyofwork.iisg.nl/resource/02> ;
    skos:definition "Workers in this unit group carry out research on electrical and electronics engineering problems, design and advise on electrical and electronic systems and equipment, plan and supervise development, construction, installation, operation, maintenance and repair of electrical and electronic equipment."@en ;
    skos:prefLabel "Electrical and Electronics Engineers"@en .

<http://historyofwork.iisg.nl/resource/030> a skos:Concept ;
    skos:broader <http://historyofwork.iisg.nl/resource/03> ;
    skos:definition "Workers in this unit group survey the earth's surface, natural topography and man-made structures, and underground areas, and prepare maps and charts. Their functions include: surveying land surfaces to determine boundaries and exact locations, delineate topographic features and otherwise measure land areas for such purposes as mapmaking and construction work; surveying mines and delineating surface and underground features to control direction and extent of mining; surveying sea, river and lake beds for such purposes as chart making, determining navigable channels and planning construction of marine structures; analysing aerial photographs to prepare or revise topographic maps and charts. Quantity surveyor is classified in 0-33.20 and valuation surveyor in unit group 4-43."@en ;
    skos:prefLabel "Surveyors"@en .

<http://historyofwork.iisg.nl/resource/035> a skos:Concept ;
    skos:broader <http://historyofwork.iisg.nl/resource/03> ;
    skos:definition "Workers in this unit group perform technical tasks, normally under the direction and supervision of mechanical engineers, contributory to the design, development, manufacture, construction, installation, maintenance and repair of mechanically functioning plant and equipment. Their functions include: assisting in research and development work concerning machine tools, engines, vehicles, aeroplanes, heating, ventilating and refrigerating installations and other mechanically functioning plant and equipment; preparing detailed estimates of quantities and costs of materials and labour required for manufacture and installation; assisting with technical supervision of manufacture, installation, maintenance and repair of mechanical plant and equipment; applying knowledge of mechanical engineering theory and practices to recognise and solve problems arising in the course of their work."@en ;
    skos:prefLabel "Mechanical Engineering Technicians"@en .

<http://historyofwork.iisg.nl/resource/041> a skos:Concept ;
    skos:broader <http://historyofwork.iisg.nl/resource/04> ;
    skos:definition "Workers in this unit group fly aircraft, direct the course of aircraft in flight, inspect, adjust and regulate during flight the mechanical equipment of aircraft and give flying instruction. Their functions include: flying aircraft to transport passengers, mail or freight; flying aircraft for testing or delivery, aerial spraying, aerial surveys or photography, and exhibitions of flying skill; navigating aircraft in flight; inspecting mechanical and other equipment of aircraft, making adjustments and minor repairs, monitoring control panel during flight and regulating engine speed according to pilot's instructions; teaching trainee pilots to fly aircraft."@en ;
    skos:prefLabel "Aircraft Pilots, Navigators and Flight Engineers"@en .

<http://historyofwork.iisg.nl/resource/053> a skos:Concept ;
    skos:broader <http://historyofwork.iisg.nl/resource/05> ;
    skos:definition "Workers in this unit group conduct research into field-crop growing, horticulture, forestry and soils and develop improved methods of propagation, cultivation, harvesting, pest control and related farming activities. Their functions include: conducting research into field and horticultural crops and forestry to develop new and improved methods giving higher yields and better quality; planning and directing forest planting, care and exploitation of forest stands; studying the characteristics, use capabilities and productivity of soils and applying findings to development of improved agricultural, horticultural and forestry practices; advising farmers on farming methods and problems."@en ;
    skos:prefLabel "Agronomists and Related Scientists"@en .

<http://historyofwork.iisg.nl/resource/061> a skos:Concept ;
    skos:broader <http://historyofwork.iisg.nl/resource/06> ;
    skos:definition "Workers in this unit group apply medical knowledge to the prevention, diagnosis and treatment of human illnesses. Their functions include: conducting medical examinations, making diagnoses, prescribing and giving treatment for diseases, disorders and injuries of the human body, and applying preventive medicine techniques; performing surgical operations in the treatment of injuries, diseases and disorders of the human body; implementing public health laws and regulations for safeguarding and promoting the health of a community; performing related tasks. Anatomists, Physiologists, Bacteriologists, Medical pathologists and Pharmacologists are classified in unit group 0-52, Dentists in 0-63 and Pharmacists in 0-67."@en ;
    skos:prefLabel "Medical Doctors"@en .

<http://historyofwork.iisg.nl/resource/042> a skos:Concept ;
    skos:broader <http://historyofwork.iisg.nl/resource/04> ;
    skos:definition "Workers in this unit group command and navigate ships and hovercraft and direct marine services on shore for shipping company vessels arriving in port. Their functions include: taking complete charge of seagoing or inland waterway vessels; planning, supervising and co-ordinating deck and bridge-watch activities on vessels; navigating vessels into and out of ports and through channels, straits and other waters where special knowledge and skill are required; directing or arranging supply of ships' stores and equipment, recruitment of crews and provision of other services (except engineering) for company vessels arriving in port."@en ;
    skos:prefLabel "Ships' Deck Officers and Pilots"@en .

<http://historyofwork.iisg.nl/resource/07> a skos:Concept ;
    skos:broader <http://historyofwork.iisg.nl/resource/0> ;
    skos:definition "Workers in this minor group diagnose, and prescribe and give medical and surgical curative and preventive treatment for, human and animal illnesses; make and dispense medicaments; provide professional and non-professional nursing services; prescribe and fit spectacles; provide special medical therapeutic services; operate X-ray equipment for medical diagnostic or therapeutic treatment purposes; and perform related tasks."@en ;
    skos:prefLabel "Medical, Dental, Veterinary And Related Workers"@en .

<http://historyofwork.iisg.nl/resource/012> a skos:Concept ;
    skos:broader <http://historyofwork.iisg.nl/resource/01> ;
    skos:definition "Workers in this unit group conduct research into physical phenomena in such fields as mechanics, heat, light, sound, electricity and magnetism, electronics and nuclear physics. Their functions include: conducting pure research to increase scientific knowledge in the field of physics; conducting applied research to develop or improve industrial, medical, military and other practical applications of the laws and theories of physics."@en ;
    skos:prefLabel "Physicists"@en .

<http://historyofwork.iisg.nl/resource/031> a skos:Concept ;
    skos:broader <http://historyofwork.iisg.nl/resource/03> ;
    skos:definition "Workers in this unit group prepare technical drawings and maps and copy drawings and paintings onto printing plates. Their functions include: preparing working drawings from designers' sketches and specifications for such purposes as manufacture and installation of machinery and equipment or for construction of buildings, bridges, dams, roads and other civil engineering projects; preparing topographical, political, economic, nautical and other maps and charts from survey and other data; drawing technical illustrations for reference works, brochures and technical manuals dealing with assembly, installation, operation, maintenance and repair of machinery and other equipment; copying drawings and paintings onto stone or metal plates for printing."@en ;
    skos:prefLabel "Draughtsmen"@en .

<http://historyofwork.iisg.nl/resource/052> a skos:Concept ;
    skos:broader <http://historyofwork.iisg.nl/resource/05> ;
    skos:definition "Workers in this unit group study the structure, composition, and life processes of humans, animals and micro-organisms and apply their findings to such purposes as prevention of disease in humans and animals, promotion of health and physical fitness and development of animals for economic exploitation. Their functions include: conducting research into the form, structure and other anatomical characteristics of humans and animals, the chemical composition and processes of living organisms, the biological functions and activities of the human organism under normal and abnormal conditions, the nature and characteristics of bacteria and their action on living organisms and dead organic matter, the nature, causes and development of human and animal diseases and parasites, effects of drugs on organs, tissues and life processes of humans and animals, and systems of selective breeding of animals and advanced methods of animal husbandry; developing practical applications of such scientific knowledge in medical public health, agricultural, industrial and other fields"@en ;
    skos:prefLabel "Bacteriologists, Pharmacologists and Related Scientists"@en .

<http://historyofwork.iisg.nl/resource/06> a skos:Concept ;
    skos:broader <http://historyofwork.iisg.nl/resource/0> ;
    skos:definition "Workers in this minor group diagnose, and prescribe and give medical and surgical curative and preventive treatment for, human and animal illnesses; make and dispense medicaments; provide professional and non-professional nursing services; prescribe and fit spectacles; provide special medical therapeutic services; operate X-ray equipment for medical diagnostic or therapeutic treatment purposes; and perform related tasks."@en ;
    skos:prefLabel "Medical, Dental, Veterinary And Related Workers"@en .

<http://historyofwork.iisg.nl/resource/02> a skos:Concept ;
    skos:broader <http://historyofwork.iisg.nl/resource/0> ;
    skos:definition "Workers in this minor group design buildings and supervise their construction; plan and co-ordinate development of urban areas; plan, design and supervise landscaping; study, design, advise on and supervise the construction of civil engineering structures; study, advise on and develop plant, equipment and processes in electrical, electronic, mechanical, chemical, mining and other engineering fields and carry out technical supervisory functions in connection with the manufacture, construction, installation, operation, maintenance and repair of such plant and equipment; develop and control processes for extraction of metals from their ores, study properties of metals, develop new alloys and advise on metallurgical problems; study, develop and advise on the promotion of efficient, safe and economic utilisation of personnel, materials and equipment; study, plan and advise on the routing and control of road traffic; make trigonometric surveys of the earth's surface and underground areas; prepare technical drawings and maps and perform other technical tasks, normally under supervision, contributory to the work described in the foregoing. Workers with architectural and engineering qualifications frequently are occupied mainly in administrative or managerial work (minor group 2-1), or as teachers (minor group 1-3), patent agents (unit group 1-99) or technical salesmen (unit group 4-31) and are classified accordingly."@en ;
    skos:prefLabel "Architects, Engineers And Related Technicians"@en .

<http://historyofwork.iisg.nl/resource/022> a skos:Concept ;
    skos:broader <http://historyofwork.iisg.nl/resource/02> ;
    skos:definition "Workers in this unit group carry out research and advise on civil engineering problems, design projects and structures such as bridges, dams, docks, roads, airports, railways, waste disposal systems, flood control systems and industrial and other large buildings, and plan, organise and supervise their construction, maintenance and repair."@en ;
    skos:prefLabel "Civil Engineers"@en .

<http://historyofwork.iisg.nl/resource/024> a skos:Concept ;
    skos:broader <http://historyofwork.iisg.nl/resource/02> ;
    skos:definition "Workers in this unit group carry out research on, design and advise on mechanically functioning plant and equipment, such as machine tools, engines, vehicles, heating, ventilating and refrigerating installations, and plant and equipment for the release, control and utilisation of nuclear energy, and plan and supervise their development, manufacture, construction, installation, operation, maintenance and repair."@en ;
    skos:prefLabel "Mechanical Engineers"@en .

<http://historyofwork.iisg.nl/resource/03> a skos:Concept ;
    skos:broader <http://historyofwork.iisg.nl/resource/0> ;
    skos:definition "Workers in this minor group design buildings and supervise their construction; plan and co-ordinate development of urban areas; plan, design and supervise landscaping; study, design, advise on and supervise the construction of civil engineering structures; study, advise on and develop plant, equipment and processes in electrical, electronic, mechanical, chemical, mining and other engineering fields and carry out technical supervisory functions in connection with the manufacture, construction, installation, operation, maintenance and repair of such plant and equipment; develop and control processes for extraction of metals from their ores, study properties of metals, develop new alloys and advise on metallurgical problems; study, develop and advise on the promotion of efficient, safe and economic utilisation of personnel, materials and equipment; study, plan and advise on the routing and control of road traffic; make trigonometric surveys of the earth's surface and underground areas; prepare technical drawings and maps and perform other technical tasks, normally under supervision, contributory to the work described in the foregoing. Workers with architectural and engineering qualifications frequently are occupied mainly in administrative or managerial work (minor group 2-1), or as teachers (minor group 1-3), patent agents (unit group 1-99) or technical salesmen (unit group 4-31) and are classified accordingly."@en ;
    skos:prefLabel "Architects, Engineers And Related Technicians"@en .

